include/s2n-bignum.h
@@ -748,6 +748,11 @@ extern void curve25519_x25519_alt(uint64_t res[static 4],uint64_t scalar[static 
 extern void curve25519_x25519base(uint64_t res[static 4],uint64_t scalar[static 4]);
 extern void curve25519_x25519base_alt(uint64_t res[static 4],uint64_t scalar[static 4]);
 
+// Extended projective addition for edwards25519
+// Inputs p1[16], p2[16]; output p3[16]
+extern void edwards25519_epadd(uint64_t p3[static 16],uint64_t p1[static 16],uint64_t p2[static 16]);
+extern void edwards25519_epadd_alt(uint64_t p3[static 16],uint64_t p1[static 16],uint64_t p2[static 16]);
+
 // Extended projective + precomputed mixed addition for edwards25519
 // Inputs p1[16], p2[12]; output p3[16]
 extern void edwards25519_pepadd(uint64_t p3[static 16],uint64_t p1[static 16],uint64_t p2[static 12]);
