arm/proofs/edwards25519_epadd.ml
@@ -4,7 +4,7 @@
  *)
 
 (* ========================================================================= *)
-(* Specialized extended projective mixed addition for edwards25519.          *)
+(* Extended projective addition for edwards25519.                            *)
 (* ========================================================================= *)
 
 needs "arm/proofs/base.ml";;
@@ -19,53 +19,19 @@ prioritize_int();;
 prioritize_real();;
 prioritize_num();;
 
-(**** print_literal_from_elf "arm/curve25519/edwards25519_pepadd.o";;
+(**** print_literal_from_elf "arm/curve25519/edwards25519_epadd.o";;
  ****)
 
-let edwards25519_pepadd_mc = define_assert_from_elf
-  "edwards25519_pepadd_mc" "arm/curve25519/edwards25519_pepadd.o"
+let edwards25519_epadd_mc = define_assert_from_elf
+  "edwards25519_epadd_mc" "arm/curve25519/edwards25519_epadd.o"
 [
   0xa9bf53f3;       (* arm_STP X19 X20 SP (Preimmediate_Offset (iword (-- &16))) *)
   0xd10303ff;       (* arm_SUB SP SP (rvalue (word 192)) *)
   0xaa0003f1;       (* arm_MOV X17 X0 *)
   0xaa0103f3;       (* arm_MOV X19 X1 *)
   0xaa0203f4;       (* arm_MOV X20 X2 *)
-  0xa9440660;       (* arm_LDP X0 X1 X19 (Immediate_Offset (iword (&64))) *)
-  0xab000000;       (* arm_ADDS X0 X0 X0 *)
-  0xba010021;       (* arm_ADCS X1 X1 X1 *)
-  0xa9450e62;       (* arm_LDP X2 X3 X19 (Immediate_Offset (iword (&80))) *)
-  0xba020042;       (* arm_ADCS X2 X2 X2 *)
-  0x9a030063;       (* arm_ADC X3 X3 X3 *)
-  0xa90007e0;       (* arm_STP X0 X1 SP (Immediate_Offset (iword (&0))) *)
-  0xa9010fe2;       (* arm_STP X2 X3 SP (Immediate_Offset (iword (&16))) *)
-  0xa9421a65;       (* arm_LDP X5 X6 X19 (Immediate_Offset (iword (&32))) *)
-  0xa9400e64;       (* arm_LDP X4 X3 X19 (Immediate_Offset (iword (&0))) *)
-  0xeb0400a5;       (* arm_SUBS X5 X5 X4 *)
-  0xfa0300c6;       (* arm_SBCS X6 X6 X3 *)
-  0xa9432267;       (* arm_LDP X7 X8 X19 (Immediate_Offset (iword (&48))) *)
-  0xa9410e64;       (* arm_LDP X4 X3 X19 (Immediate_Offset (iword (&16))) *)
-  0xfa0400e7;       (* arm_SBCS X7 X7 X4 *)
-  0xfa030108;       (* arm_SBCS X8 X8 X3 *)
-  0xd2800263;       (* arm_MOV X3 (rvalue (word 19)) *)
-  0xeb0300a5;       (* arm_SUBS X5 X5 X3 *)
-  0xfa1f00c6;       (* arm_SBCS X6 X6 XZR *)
-  0xfa1f00e7;       (* arm_SBCS X7 X7 XZR *)
-  0xd2f00004;       (* arm_MOVZ X4 (word 32768) 48 *)
-  0xda040108;       (* arm_SBC X8 X8 X4 *)
-  0xa9021be5;       (* arm_STP X5 X6 SP (Immediate_Offset (iword (&32))) *)
-  0xa90323e7;       (* arm_STP X7 X8 SP (Immediate_Offset (iword (&48))) *)
-  0xa9420660;       (* arm_LDP X0 X1 X19 (Immediate_Offset (iword (&32))) *)
-  0xa9401664;       (* arm_LDP X4 X5 X19 (Immediate_Offset (iword (&0))) *)
-  0xab040000;       (* arm_ADDS X0 X0 X4 *)
-  0xba050021;       (* arm_ADCS X1 X1 X5 *)
-  0xa9430e62;       (* arm_LDP X2 X3 X19 (Immediate_Offset (iword (&48))) *)
-  0xa9411e66;       (* arm_LDP X6 X7 X19 (Immediate_Offset (iword (&16))) *)
-  0xba060042;       (* arm_ADCS X2 X2 X6 *)
-  0x9a070063;       (* arm_ADC X3 X3 X7 *)
-  0xa90407e0;       (* arm_STP X0 X1 SP (Immediate_Offset (iword (&64))) *)
-  0xa9050fe2;       (* arm_STP X2 X3 SP (Immediate_Offset (iword (&80))) *)
   0xa9461263;       (* arm_LDP X3 X4 X19 (Immediate_Offset (iword (&96))) *)
-  0xa9441a85;       (* arm_LDP X5 X6 X20 (Immediate_Offset (iword (&64))) *)
+  0xa9461a85;       (* arm_LDP X5 X6 X20 (Immediate_Offset (iword (&96))) *)
   0x9b057c67;       (* arm_MUL X7 X3 X5 *)
   0x9bc57c68;       (* arm_UMULH X8 X3 X5 *)
   0x9b067c89;       (* arm_MUL X9 X4 X6 *)
@@ -90,7 +56,7 @@ let edwards25519_pepadd_mc = define_assert_from_elf
   0xba090069;       (* arm_ADCS X9 X3 X9 *)
   0x9a10014a;       (* arm_ADC X10 X10 X16 *)
   0xa9471263;       (* arm_LDP X3 X4 X19 (Immediate_Offset (iword (&112))) *)
-  0xa9451a85;       (* arm_LDP X5 X6 X20 (Immediate_Offset (iword (&80))) *)
+  0xa9471a85;       (* arm_LDP X5 X6 X20 (Immediate_Offset (iword (&112))) *)
   0x9b057c6b;       (* arm_MUL X11 X3 X5 *)
   0x9bc57c6c;       (* arm_UMULH X12 X3 X5 *)
   0x9b067c8d;       (* arm_MUL X13 X4 X6 *)
@@ -119,7 +85,7 @@ let edwards25519_pepadd_mc = define_assert_from_elf
   0xeb0f0063;       (* arm_SUBS X3 X3 X15 *)
   0xfa100084;       (* arm_SBCS X4 X4 X16 *)
   0xda9f23f0;       (* arm_CSETM X16 Condition_CC *)
-  0xa944028f;       (* arm_LDP X15 X0 X20 (Immediate_Offset (iword (&64))) *)
+  0xa946028f;       (* arm_LDP X15 X0 X20 (Immediate_Offset (iword (&96))) *)
   0xeb0501e5;       (* arm_SUBS X5 X15 X5 *)
   0xfa060006;       (* arm_SBCS X6 X0 X6 *)
   0xda9f23e0;       (* arm_CSETM X0 Condition_CC *)
@@ -217,10 +183,70 @@ let edwards25519_pepadd_mc = define_assert_from_elf
   0xba1f0108;       (* arm_ADCS X8 X8 XZR *)
   0xba1f0129;       (* arm_ADCS X9 X9 XZR *)
   0x9a1f014a;       (* arm_ADC X10 X10 XZR *)
-  0xa90623e7;       (* arm_STP X7 X8 SP (Immediate_Offset (iword (&96))) *)
-  0xa9072be9;       (* arm_STP X9 X10 SP (Immediate_Offset (iword (&112))) *)
+  0xa90023e7;       (* arm_STP X7 X8 SP (Immediate_Offset (iword (&0))) *)
+  0xa9012be9;       (* arm_STP X9 X10 SP (Immediate_Offset (iword (&16))) *)
+  0xa9421a65;       (* arm_LDP X5 X6 X19 (Immediate_Offset (iword (&32))) *)
+  0xa9400e64;       (* arm_LDP X4 X3 X19 (Immediate_Offset (iword (&0))) *)
+  0xeb0400a5;       (* arm_SUBS X5 X5 X4 *)
+  0xfa0300c6;       (* arm_SBCS X6 X6 X3 *)
+  0xa9432267;       (* arm_LDP X7 X8 X19 (Immediate_Offset (iword (&48))) *)
+  0xa9410e64;       (* arm_LDP X4 X3 X19 (Immediate_Offset (iword (&16))) *)
+  0xfa0400e7;       (* arm_SBCS X7 X7 X4 *)
+  0xfa030108;       (* arm_SBCS X8 X8 X3 *)
+  0xd2800263;       (* arm_MOV X3 (rvalue (word 19)) *)
+  0xeb0300a5;       (* arm_SUBS X5 X5 X3 *)
+  0xfa1f00c6;       (* arm_SBCS X6 X6 XZR *)
+  0xfa1f00e7;       (* arm_SBCS X7 X7 XZR *)
+  0xd2f00004;       (* arm_MOVZ X4 (word 32768) 48 *)
+  0xda040108;       (* arm_SBC X8 X8 X4 *)
+  0xa9021be5;       (* arm_STP X5 X6 SP (Immediate_Offset (iword (&32))) *)
+  0xa90323e7;       (* arm_STP X7 X8 SP (Immediate_Offset (iword (&48))) *)
+  0xa9421a85;       (* arm_LDP X5 X6 X20 (Immediate_Offset (iword (&32))) *)
+  0xa9400e84;       (* arm_LDP X4 X3 X20 (Immediate_Offset (iword (&0))) *)
+  0xeb0400a5;       (* arm_SUBS X5 X5 X4 *)
+  0xfa0300c6;       (* arm_SBCS X6 X6 X3 *)
+  0xa9432287;       (* arm_LDP X7 X8 X20 (Immediate_Offset (iword (&48))) *)
+  0xa9410e84;       (* arm_LDP X4 X3 X20 (Immediate_Offset (iword (&16))) *)
+  0xfa0400e7;       (* arm_SBCS X7 X7 X4 *)
+  0xfa030108;       (* arm_SBCS X8 X8 X3 *)
+  0xd2800263;       (* arm_MOV X3 (rvalue (word 19)) *)
+  0xeb0300a5;       (* arm_SUBS X5 X5 X3 *)
+  0xfa1f00c6;       (* arm_SBCS X6 X6 XZR *)
+  0xfa1f00e7;       (* arm_SBCS X7 X7 XZR *)
+  0xd2f00004;       (* arm_MOVZ X4 (word 32768) 48 *)
+  0xda040108;       (* arm_SBC X8 X8 X4 *)
+  0xa9041be5;       (* arm_STP X5 X6 SP (Immediate_Offset (iword (&64))) *)
+  0xa90523e7;       (* arm_STP X7 X8 SP (Immediate_Offset (iword (&80))) *)
+  0xa9420660;       (* arm_LDP X0 X1 X19 (Immediate_Offset (iword (&32))) *)
+  0xa9401664;       (* arm_LDP X4 X5 X19 (Immediate_Offset (iword (&0))) *)
+  0xab040000;       (* arm_ADDS X0 X0 X4 *)
+  0xba050021;       (* arm_ADCS X1 X1 X5 *)
+  0xa9430e62;       (* arm_LDP X2 X3 X19 (Immediate_Offset (iword (&48))) *)
+  0xa9411e66;       (* arm_LDP X6 X7 X19 (Immediate_Offset (iword (&16))) *)
+  0xba060042;       (* arm_ADCS X2 X2 X6 *)
+  0x9a070063;       (* arm_ADC X3 X3 X7 *)
+  0xa90607e0;       (* arm_STP X0 X1 SP (Immediate_Offset (iword (&96))) *)
+  0xa9070fe2;       (* arm_STP X2 X3 SP (Immediate_Offset (iword (&112))) *)
+  0xa9420680;       (* arm_LDP X0 X1 X20 (Immediate_Offset (iword (&32))) *)
+  0xa9401684;       (* arm_LDP X4 X5 X20 (Immediate_Offset (iword (&0))) *)
+  0xab040000;       (* arm_ADDS X0 X0 X4 *)
+  0xba050021;       (* arm_ADCS X1 X1 X5 *)
+  0xa9430e82;       (* arm_LDP X2 X3 X20 (Immediate_Offset (iword (&48))) *)
+  0xa9411e86;       (* arm_LDP X6 X7 X20 (Immediate_Offset (iword (&16))) *)
+  0xba060042;       (* arm_ADCS X2 X2 X6 *)
+  0x9a070063;       (* arm_ADC X3 X3 X7 *)
+  0xa90807e0;       (* arm_STP X0 X1 SP (Immediate_Offset (iword (&128))) *)
+  0xa9090fe2;       (* arm_STP X2 X3 SP (Immediate_Offset (iword (&144))) *)
+  0xa9440680;       (* arm_LDP X0 X1 X20 (Immediate_Offset (iword (&64))) *)
+  0xab000000;       (* arm_ADDS X0 X0 X0 *)
+  0xba010021;       (* arm_ADCS X1 X1 X1 *)
+  0xa9450e82;       (* arm_LDP X2 X3 X20 (Immediate_Offset (iword (&80))) *)
+  0xba020042;       (* arm_ADCS X2 X2 X2 *)
+  0x9a030063;       (* arm_ADC X3 X3 X3 *)
+  0xa90a07e0;       (* arm_STP X0 X1 SP (Immediate_Offset (iword (&160))) *)
+  0xa90b0fe2;       (* arm_STP X2 X3 SP (Immediate_Offset (iword (&176))) *)
   0xa94213e3;       (* arm_LDP X3 X4 SP (Immediate_Offset (iword (&32))) *)
-  0xa9401a85;       (* arm_LDP X5 X6 X20 (Immediate_Offset (iword (&0))) *)
+  0xa9441be5;       (* arm_LDP X5 X6 SP (Immediate_Offset (iword (&64))) *)
   0x9b057c67;       (* arm_MUL X7 X3 X5 *)
   0x9bc57c68;       (* arm_UMULH X8 X3 X5 *)
   0x9b067c89;       (* arm_MUL X9 X4 X6 *)
@@ -245,7 +271,7 @@ let edwards25519_pepadd_mc = define_assert_from_elf
   0xba090069;       (* arm_ADCS X9 X3 X9 *)
   0x9a10014a;       (* arm_ADC X10 X10 X16 *)
   0xa94313e3;       (* arm_LDP X3 X4 SP (Immediate_Offset (iword (&48))) *)
-  0xa9411a85;       (* arm_LDP X5 X6 X20 (Immediate_Offset (iword (&16))) *)
+  0xa9451be5;       (* arm_LDP X5 X6 SP (Immediate_Offset (iword (&80))) *)
   0x9b057c6b;       (* arm_MUL X11 X3 X5 *)
   0x9bc57c6c;       (* arm_UMULH X12 X3 X5 *)
   0x9b067c8d;       (* arm_MUL X13 X4 X6 *)
@@ -274,7 +300,7 @@ let edwards25519_pepadd_mc = define_assert_from_elf
   0xeb0f0063;       (* arm_SUBS X3 X3 X15 *)
   0xfa100084;       (* arm_SBCS X4 X4 X16 *)
   0xda9f23f0;       (* arm_CSETM X16 Condition_CC *)
-  0xa940028f;       (* arm_LDP X15 X0 X20 (Immediate_Offset (iword (&0))) *)
+  0xa94403ef;       (* arm_LDP X15 X0 SP (Immediate_Offset (iword (&64))) *)
   0xeb0501e5;       (* arm_SUBS X5 X15 X5 *)
   0xfa060006;       (* arm_SBCS X6 X0 X6 *)
   0xda9f23e0;       (* arm_CSETM X0 Condition_CC *)
@@ -374,8 +400,181 @@ let edwards25519_pepadd_mc = define_assert_from_elf
   0x9a1f014a;       (* arm_ADC X10 X10 XZR *)
   0xa90223e7;       (* arm_STP X7 X8 SP (Immediate_Offset (iword (&32))) *)
   0xa9032be9;       (* arm_STP X9 X10 SP (Immediate_Offset (iword (&48))) *)
+  0xa94613e3;       (* arm_LDP X3 X4 SP (Immediate_Offset (iword (&96))) *)
+  0xa9481be5;       (* arm_LDP X5 X6 SP (Immediate_Offset (iword (&128))) *)
+  0x9b057c67;       (* arm_MUL X7 X3 X5 *)
+  0x9bc57c68;       (* arm_UMULH X8 X3 X5 *)
+  0x9b067c89;       (* arm_MUL X9 X4 X6 *)
+  0x9bc67c8a;       (* arm_UMULH X10 X4 X6 *)
+  0xeb030084;       (* arm_SUBS X4 X4 X3 *)
+  0xda842484;       (* arm_CNEG X4 X4 Condition_CC *)
+  0xda9f23f0;       (* arm_CSETM X16 Condition_CC *)
+  0xab080129;       (* arm_ADDS X9 X9 X8 *)
+  0x9a1f014a;       (* arm_ADC X10 X10 XZR *)
+  0xeb0600a3;       (* arm_SUBS X3 X5 X6 *)
+  0xda832463;       (* arm_CNEG X3 X3 Condition_CC *)
+  0xda902210;       (* arm_CINV X16 X16 Condition_CC *)
+  0x9b037c8f;       (* arm_MUL X15 X4 X3 *)
+  0x9bc37c83;       (* arm_UMULH X3 X4 X3 *)
+  0xab0900e8;       (* arm_ADDS X8 X7 X9 *)
+  0xba0a0129;       (* arm_ADCS X9 X9 X10 *)
+  0x9a1f014a;       (* arm_ADC X10 X10 XZR *)
+  0xb100061f;       (* arm_CMN X16 (rvalue (word 1)) *)
+  0xca1001ef;       (* arm_EOR X15 X15 X16 *)
+  0xba0801e8;       (* arm_ADCS X8 X15 X8 *)
+  0xca100063;       (* arm_EOR X3 X3 X16 *)
+  0xba090069;       (* arm_ADCS X9 X3 X9 *)
+  0x9a10014a;       (* arm_ADC X10 X10 X16 *)
+  0xa94713e3;       (* arm_LDP X3 X4 SP (Immediate_Offset (iword (&112))) *)
+  0xa9491be5;       (* arm_LDP X5 X6 SP (Immediate_Offset (iword (&144))) *)
+  0x9b057c6b;       (* arm_MUL X11 X3 X5 *)
+  0x9bc57c6c;       (* arm_UMULH X12 X3 X5 *)
+  0x9b067c8d;       (* arm_MUL X13 X4 X6 *)
+  0x9bc67c8e;       (* arm_UMULH X14 X4 X6 *)
+  0xeb030084;       (* arm_SUBS X4 X4 X3 *)
+  0xda842484;       (* arm_CNEG X4 X4 Condition_CC *)
+  0xda9f23f0;       (* arm_CSETM X16 Condition_CC *)
+  0xab0c01ad;       (* arm_ADDS X13 X13 X12 *)
+  0x9a1f01ce;       (* arm_ADC X14 X14 XZR *)
+  0xeb0600a3;       (* arm_SUBS X3 X5 X6 *)
+  0xda832463;       (* arm_CNEG X3 X3 Condition_CC *)
+  0xda902210;       (* arm_CINV X16 X16 Condition_CC *)
+  0x9b037c8f;       (* arm_MUL X15 X4 X3 *)
+  0x9bc37c83;       (* arm_UMULH X3 X4 X3 *)
+  0xab0d016c;       (* arm_ADDS X12 X11 X13 *)
+  0xba0e01ad;       (* arm_ADCS X13 X13 X14 *)
+  0x9a1f01ce;       (* arm_ADC X14 X14 XZR *)
+  0xb100061f;       (* arm_CMN X16 (rvalue (word 1)) *)
+  0xca1001ef;       (* arm_EOR X15 X15 X16 *)
+  0xba0c01ec;       (* arm_ADCS X12 X15 X12 *)
+  0xca100063;       (* arm_EOR X3 X3 X16 *)
+  0xba0d006d;       (* arm_ADCS X13 X3 X13 *)
+  0x9a1001ce;       (* arm_ADC X14 X14 X16 *)
+  0xa94713e3;       (* arm_LDP X3 X4 SP (Immediate_Offset (iword (&112))) *)
+  0xa94643ef;       (* arm_LDP X15 X16 SP (Immediate_Offset (iword (&96))) *)
+  0xeb0f0063;       (* arm_SUBS X3 X3 X15 *)
+  0xfa100084;       (* arm_SBCS X4 X4 X16 *)
+  0xda9f23f0;       (* arm_CSETM X16 Condition_CC *)
+  0xa94803ef;       (* arm_LDP X15 X0 SP (Immediate_Offset (iword (&128))) *)
+  0xeb0501e5;       (* arm_SUBS X5 X15 X5 *)
+  0xfa060006;       (* arm_SBCS X6 X0 X6 *)
+  0xda9f23e0;       (* arm_CSETM X0 Condition_CC *)
+  0xca100063;       (* arm_EOR X3 X3 X16 *)
+  0xeb100063;       (* arm_SUBS X3 X3 X16 *)
+  0xca100084;       (* arm_EOR X4 X4 X16 *)
+  0xda100084;       (* arm_SBC X4 X4 X16 *)
+  0xca0000a5;       (* arm_EOR X5 X5 X0 *)
+  0xeb0000a5;       (* arm_SUBS X5 X5 X0 *)
+  0xca0000c6;       (* arm_EOR X6 X6 X0 *)
+  0xda0000c6;       (* arm_SBC X6 X6 X0 *)
+  0xca100010;       (* arm_EOR X16 X0 X16 *)
+  0xab09016b;       (* arm_ADDS X11 X11 X9 *)
+  0xba0a018c;       (* arm_ADCS X12 X12 X10 *)
+  0xba1f01ad;       (* arm_ADCS X13 X13 XZR *)
+  0x9a1f01ce;       (* arm_ADC X14 X14 XZR *)
+  0x9b057c62;       (* arm_MUL X2 X3 X5 *)
+  0x9bc57c60;       (* arm_UMULH X0 X3 X5 *)
+  0x9b067c8f;       (* arm_MUL X15 X4 X6 *)
+  0x9bc67c81;       (* arm_UMULH X1 X4 X6 *)
+  0xeb030084;       (* arm_SUBS X4 X4 X3 *)
+  0xda842484;       (* arm_CNEG X4 X4 Condition_CC *)
+  0xda9f23e9;       (* arm_CSETM X9 Condition_CC *)
+  0xab0001ef;       (* arm_ADDS X15 X15 X0 *)
+  0x9a1f0021;       (* arm_ADC X1 X1 XZR *)
+  0xeb0600a6;       (* arm_SUBS X6 X5 X6 *)
+  0xda8624c6;       (* arm_CNEG X6 X6 Condition_CC *)
+  0xda892129;       (* arm_CINV X9 X9 Condition_CC *)
+  0x9b067c85;       (* arm_MUL X5 X4 X6 *)
+  0x9bc67c86;       (* arm_UMULH X6 X4 X6 *)
+  0xab0f0040;       (* arm_ADDS X0 X2 X15 *)
+  0xba0101ef;       (* arm_ADCS X15 X15 X1 *)
+  0x9a1f0021;       (* arm_ADC X1 X1 XZR *)
+  0xb100053f;       (* arm_CMN X9 (rvalue (word 1)) *)
+  0xca0900a5;       (* arm_EOR X5 X5 X9 *)
+  0xba0000a0;       (* arm_ADCS X0 X5 X0 *)
+  0xca0900c6;       (* arm_EOR X6 X6 X9 *)
+  0xba0f00cf;       (* arm_ADCS X15 X6 X15 *)
+  0x9a090021;       (* arm_ADC X1 X1 X9 *)
+  0xab070169;       (* arm_ADDS X9 X11 X7 *)
+  0xba08018a;       (* arm_ADCS X10 X12 X8 *)
+  0xba0b01ab;       (* arm_ADCS X11 X13 X11 *)
+  0xba0c01cc;       (* arm_ADCS X12 X14 X12 *)
+  0xba1f01ad;       (* arm_ADCS X13 X13 XZR *)
+  0x9a1f01ce;       (* arm_ADC X14 X14 XZR *)
+  0xb100061f;       (* arm_CMN X16 (rvalue (word 1)) *)
+  0xca100042;       (* arm_EOR X2 X2 X16 *)
+  0xba090049;       (* arm_ADCS X9 X2 X9 *)
+  0xca100000;       (* arm_EOR X0 X0 X16 *)
+  0xba0a000a;       (* arm_ADCS X10 X0 X10 *)
+  0xca1001ef;       (* arm_EOR X15 X15 X16 *)
+  0xba0b01eb;       (* arm_ADCS X11 X15 X11 *)
+  0xca100021;       (* arm_EOR X1 X1 X16 *)
+  0xba0c002c;       (* arm_ADCS X12 X1 X12 *)
+  0xba1001ad;       (* arm_ADCS X13 X13 X16 *)
+  0x9a1001ce;       (* arm_ADC X14 X14 X16 *)
+  0xd28004c3;       (* arm_MOV X3 (rvalue (word 38)) *)
+  0x92407d65;       (* arm_AND X5 X11 (rvalue (word 4294967295)) *)
+  0xd360fd64;       (* arm_LSR X4 X11 32 *)
+  0x9b057c65;       (* arm_MUL X5 X3 X5 *)
+  0x9b047c64;       (* arm_MUL X4 X3 X4 *)
+  0xab0500e7;       (* arm_ADDS X7 X7 X5 *)
+  0x92407d85;       (* arm_AND X5 X12 (rvalue (word 4294967295)) *)
+  0xd360fd8c;       (* arm_LSR X12 X12 32 *)
+  0x9b057c65;       (* arm_MUL X5 X3 X5 *)
+  0x9b0c7c6c;       (* arm_MUL X12 X3 X12 *)
+  0xba050108;       (* arm_ADCS X8 X8 X5 *)
+  0x92407da5;       (* arm_AND X5 X13 (rvalue (word 4294967295)) *)
+  0xd360fdad;       (* arm_LSR X13 X13 32 *)
+  0x9b057c65;       (* arm_MUL X5 X3 X5 *)
+  0x9b0d7c6d;       (* arm_MUL X13 X3 X13 *)
+  0xba050129;       (* arm_ADCS X9 X9 X5 *)
+  0x92407dc5;       (* arm_AND X5 X14 (rvalue (word 4294967295)) *)
+  0xd360fdce;       (* arm_LSR X14 X14 32 *)
+  0x9b057c65;       (* arm_MUL X5 X3 X5 *)
+  0x9b0e7c6e;       (* arm_MUL X14 X3 X14 *)
+  0xba05014a;       (* arm_ADCS X10 X10 X5 *)
+  0x9a9f37eb;       (* arm_CSET X11 Condition_CS *)
+  0xd3607c85;       (* arm_LSL X5 X4 32 *)
+  0xab0500e7;       (* arm_ADDS X7 X7 X5 *)
+  0x93c48185;       (* arm_EXTR X5 X12 X4 32 *)
+  0xba050108;       (* arm_ADCS X8 X8 X5 *)
+  0x93cc81a5;       (* arm_EXTR X5 X13 X12 32 *)
+  0xba050129;       (* arm_ADCS X9 X9 X5 *)
+  0x93cd81c5;       (* arm_EXTR X5 X14 X13 32 *)
+  0xba05014a;       (* arm_ADCS X10 X10 X5 *)
+  0xd360fdc5;       (* arm_LSR X5 X14 32 *)
+  0x9a05016b;       (* arm_ADC X11 X11 X5 *)
+  0xab0a015f;       (* arm_CMN X10 X10 *)
+  0x9240f94a;       (* arm_AND X10 X10 (rvalue (word 9223372036854775807)) *)
+  0x9a0b0160;       (* arm_ADC X0 X11 X11 *)
+  0xd2800263;       (* arm_MOV X3 (rvalue (word 19)) *)
+  0x9b007c65;       (* arm_MUL X5 X3 X0 *)
+  0xab0500e7;       (* arm_ADDS X7 X7 X5 *)
+  0xba1f0108;       (* arm_ADCS X8 X8 XZR *)
+  0xba1f0129;       (* arm_ADCS X9 X9 XZR *)
+  0x9a1f014a;       (* arm_ADC X10 X10 XZR *)
+  0xa90623e7;       (* arm_STP X7 X8 SP (Immediate_Offset (iword (&96))) *)
+  0xa9072be9;       (* arm_STP X9 X10 SP (Immediate_Offset (iword (&112))) *)
+  0xd29e2b20;       (* arm_MOV X0 (rvalue (word 61785)) *)
+  0xd2962ac1;       (* arm_MOV X1 (rvalue (word 45398)) *)
+  0xd29a2602;       (* arm_MOV X2 (rvalue (word 53552)) *)
+  0xd29f9ce3;       (* arm_MOV X3 (rvalue (word 64743)) *)
+  0xf2a4d640;       (* arm_MOVK X0 (word 9906) 16 *)
+  0xf2b05061;       (* arm_MOVK X1 (word 33411) 16 *)
+  0xf2bdde62;       (* arm_MOVK X2 (word 61171) 16 *)
+  0xf2aadbe3;       (* arm_MOVK X3 (word 22239) 16 *)
+  0xf2d37280;       (* arm_MOVK X0 (word 39828) 32 *)
+  0xf2c29341;       (* arm_MOVK X1 (word 5274) 32 *)
+  0xf2d01e42;       (* arm_MOVK X2 (word 33010) 32 *)
+  0xf2db3b83;       (* arm_MOVK X3 (word 55772) 32 *)
+  0xf2fd7ac0;       (* arm_MOVK X0 (word 60374) 48 *)
+  0xf2e01c01;       (* arm_MOVK X1 (word 224) 48 *)
+  0xf2e331c2;       (* arm_MOVK X2 (word 6542) 48 *)
+  0xf2e480c3;       (* arm_MOVK X3 (word 9222) 48 *)
+  0xa90407e0;       (* arm_STP X0 X1 SP (Immediate_Offset (iword (&64))) *)
+  0xa9050fe2;       (* arm_STP X2 X3 SP (Immediate_Offset (iword (&80))) *)
   0xa94413e3;       (* arm_LDP X3 X4 SP (Immediate_Offset (iword (&64))) *)
-  0xa9421a85;       (* arm_LDP X5 X6 X20 (Immediate_Offset (iword (&32))) *)
+  0xa9401be5;       (* arm_LDP X5 X6 SP (Immediate_Offset (iword (&0))) *)
   0x9b057c67;       (* arm_MUL X7 X3 X5 *)
   0x9bc57c68;       (* arm_UMULH X8 X3 X5 *)
   0x9b067c89;       (* arm_MUL X9 X4 X6 *)
@@ -400,7 +599,7 @@ let edwards25519_pepadd_mc = define_assert_from_elf
   0xba090069;       (* arm_ADCS X9 X3 X9 *)
   0x9a10014a;       (* arm_ADC X10 X10 X16 *)
   0xa94513e3;       (* arm_LDP X3 X4 SP (Immediate_Offset (iword (&80))) *)
-  0xa9431a85;       (* arm_LDP X5 X6 X20 (Immediate_Offset (iword (&48))) *)
+  0xa9411be5;       (* arm_LDP X5 X6 SP (Immediate_Offset (iword (&16))) *)
   0x9b057c6b;       (* arm_MUL X11 X3 X5 *)
   0x9bc57c6c;       (* arm_UMULH X12 X3 X5 *)
   0x9b067c8d;       (* arm_MUL X13 X4 X6 *)
@@ -429,7 +628,7 @@ let edwards25519_pepadd_mc = define_assert_from_elf
   0xeb0f0063;       (* arm_SUBS X3 X3 X15 *)
   0xfa100084;       (* arm_SBCS X4 X4 X16 *)
   0xda9f23f0;       (* arm_CSETM X16 Condition_CC *)
-  0xa942028f;       (* arm_LDP X15 X0 X20 (Immediate_Offset (iword (&32))) *)
+  0xa94003ef;       (* arm_LDP X15 X0 SP (Immediate_Offset (iword (&0))) *)
   0xeb0501e5;       (* arm_SUBS X5 X15 X5 *)
   0xfa060006;       (* arm_SBCS X6 X0 X6 *)
   0xda9f23e0;       (* arm_CSETM X0 Condition_CC *)
@@ -529,43 +728,166 @@ let edwards25519_pepadd_mc = define_assert_from_elf
   0x9a1f014a;       (* arm_ADC X10 X10 XZR *)
   0xa90423e7;       (* arm_STP X7 X8 SP (Immediate_Offset (iword (&64))) *)
   0xa9052be9;       (* arm_STP X9 X10 SP (Immediate_Offset (iword (&80))) *)
-  0xa9401be5;       (* arm_LDP X5 X6 SP (Immediate_Offset (iword (&0))) *)
-  0xa9460fe4;       (* arm_LDP X4 X3 SP (Immediate_Offset (iword (&96))) *)
-  0xeb0400a5;       (* arm_SUBS X5 X5 X4 *)
-  0xfa0300c6;       (* arm_SBCS X6 X6 X3 *)
-  0xa94123e7;       (* arm_LDP X7 X8 SP (Immediate_Offset (iword (&16))) *)
-  0xa9470fe4;       (* arm_LDP X4 X3 SP (Immediate_Offset (iword (&112))) *)
-  0xfa0400e7;       (* arm_SBCS X7 X7 X4 *)
-  0xfa030108;       (* arm_SBCS X8 X8 X3 *)
-  0xd28004c4;       (* arm_MOV X4 (rvalue (word 38)) *)
-  0x9a9f3083;       (* arm_CSEL X3 X4 XZR Condition_CC *)
-  0xeb0300a5;       (* arm_SUBS X5 X5 X3 *)
-  0xfa1f00c6;       (* arm_SBCS X6 X6 XZR *)
-  0xfa1f00e7;       (* arm_SBCS X7 X7 XZR *)
-  0xda1f0108;       (* arm_SBC X8 X8 XZR *)
-  0xa9081be5;       (* arm_STP X5 X6 SP (Immediate_Offset (iword (&128))) *)
-  0xa90923e7;       (* arm_STP X7 X8 SP (Immediate_Offset (iword (&144))) *)
-  0xa94013e3;       (* arm_LDP X3 X4 SP (Immediate_Offset (iword (&0))) *)
-  0xa94623e7;       (* arm_LDP X7 X8 SP (Immediate_Offset (iword (&96))) *)
-  0xab070063;       (* arm_ADDS X3 X3 X7 *)
-  0xba080084;       (* arm_ADCS X4 X4 X8 *)
-  0xa9411be5;       (* arm_LDP X5 X6 SP (Immediate_Offset (iword (&16))) *)
-  0xa94723e7;       (* arm_LDP X7 X8 SP (Immediate_Offset (iword (&112))) *)
-  0xba0700a5;       (* arm_ADCS X5 X5 X7 *)
-  0xba0800c6;       (* arm_ADCS X6 X6 X8 *)
-  0xd28004c9;       (* arm_MOV X9 (rvalue (word 38)) *)
-  0x9a9f2129;       (* arm_CSEL X9 X9 XZR Condition_CS *)
-  0xab090063;       (* arm_ADDS X3 X3 X9 *)
-  0xba1f0084;       (* arm_ADCS X4 X4 XZR *)
-  0xba1f00a5;       (* arm_ADCS X5 X5 XZR *)
-  0x9a1f00c6;       (* arm_ADC X6 X6 XZR *)
-  0xa90013e3;       (* arm_STP X3 X4 SP (Immediate_Offset (iword (&0))) *)
-  0xa9011be5;       (* arm_STP X5 X6 SP (Immediate_Offset (iword (&16))) *)
-  0xa9441be5;       (* arm_LDP X5 X6 SP (Immediate_Offset (iword (&64))) *)
+  0xa9441263;       (* arm_LDP X3 X4 X19 (Immediate_Offset (iword (&64))) *)
+  0xa94a1be5;       (* arm_LDP X5 X6 SP (Immediate_Offset (iword (&160))) *)
+  0x9b057c67;       (* arm_MUL X7 X3 X5 *)
+  0x9bc57c68;       (* arm_UMULH X8 X3 X5 *)
+  0x9b067c89;       (* arm_MUL X9 X4 X6 *)
+  0x9bc67c8a;       (* arm_UMULH X10 X4 X6 *)
+  0xeb030084;       (* arm_SUBS X4 X4 X3 *)
+  0xda842484;       (* arm_CNEG X4 X4 Condition_CC *)
+  0xda9f23f0;       (* arm_CSETM X16 Condition_CC *)
+  0xab080129;       (* arm_ADDS X9 X9 X8 *)
+  0x9a1f014a;       (* arm_ADC X10 X10 XZR *)
+  0xeb0600a3;       (* arm_SUBS X3 X5 X6 *)
+  0xda832463;       (* arm_CNEG X3 X3 Condition_CC *)
+  0xda902210;       (* arm_CINV X16 X16 Condition_CC *)
+  0x9b037c8f;       (* arm_MUL X15 X4 X3 *)
+  0x9bc37c83;       (* arm_UMULH X3 X4 X3 *)
+  0xab0900e8;       (* arm_ADDS X8 X7 X9 *)
+  0xba0a0129;       (* arm_ADCS X9 X9 X10 *)
+  0x9a1f014a;       (* arm_ADC X10 X10 XZR *)
+  0xb100061f;       (* arm_CMN X16 (rvalue (word 1)) *)
+  0xca1001ef;       (* arm_EOR X15 X15 X16 *)
+  0xba0801e8;       (* arm_ADCS X8 X15 X8 *)
+  0xca100063;       (* arm_EOR X3 X3 X16 *)
+  0xba090069;       (* arm_ADCS X9 X3 X9 *)
+  0x9a10014a;       (* arm_ADC X10 X10 X16 *)
+  0xa9451263;       (* arm_LDP X3 X4 X19 (Immediate_Offset (iword (&80))) *)
+  0xa94b1be5;       (* arm_LDP X5 X6 SP (Immediate_Offset (iword (&176))) *)
+  0x9b057c6b;       (* arm_MUL X11 X3 X5 *)
+  0x9bc57c6c;       (* arm_UMULH X12 X3 X5 *)
+  0x9b067c8d;       (* arm_MUL X13 X4 X6 *)
+  0x9bc67c8e;       (* arm_UMULH X14 X4 X6 *)
+  0xeb030084;       (* arm_SUBS X4 X4 X3 *)
+  0xda842484;       (* arm_CNEG X4 X4 Condition_CC *)
+  0xda9f23f0;       (* arm_CSETM X16 Condition_CC *)
+  0xab0c01ad;       (* arm_ADDS X13 X13 X12 *)
+  0x9a1f01ce;       (* arm_ADC X14 X14 XZR *)
+  0xeb0600a3;       (* arm_SUBS X3 X5 X6 *)
+  0xda832463;       (* arm_CNEG X3 X3 Condition_CC *)
+  0xda902210;       (* arm_CINV X16 X16 Condition_CC *)
+  0x9b037c8f;       (* arm_MUL X15 X4 X3 *)
+  0x9bc37c83;       (* arm_UMULH X3 X4 X3 *)
+  0xab0d016c;       (* arm_ADDS X12 X11 X13 *)
+  0xba0e01ad;       (* arm_ADCS X13 X13 X14 *)
+  0x9a1f01ce;       (* arm_ADC X14 X14 XZR *)
+  0xb100061f;       (* arm_CMN X16 (rvalue (word 1)) *)
+  0xca1001ef;       (* arm_EOR X15 X15 X16 *)
+  0xba0c01ec;       (* arm_ADCS X12 X15 X12 *)
+  0xca100063;       (* arm_EOR X3 X3 X16 *)
+  0xba0d006d;       (* arm_ADCS X13 X3 X13 *)
+  0x9a1001ce;       (* arm_ADC X14 X14 X16 *)
+  0xa9451263;       (* arm_LDP X3 X4 X19 (Immediate_Offset (iword (&80))) *)
+  0xa944426f;       (* arm_LDP X15 X16 X19 (Immediate_Offset (iword (&64))) *)
+  0xeb0f0063;       (* arm_SUBS X3 X3 X15 *)
+  0xfa100084;       (* arm_SBCS X4 X4 X16 *)
+  0xda9f23f0;       (* arm_CSETM X16 Condition_CC *)
+  0xa94a03ef;       (* arm_LDP X15 X0 SP (Immediate_Offset (iword (&160))) *)
+  0xeb0501e5;       (* arm_SUBS X5 X15 X5 *)
+  0xfa060006;       (* arm_SBCS X6 X0 X6 *)
+  0xda9f23e0;       (* arm_CSETM X0 Condition_CC *)
+  0xca100063;       (* arm_EOR X3 X3 X16 *)
+  0xeb100063;       (* arm_SUBS X3 X3 X16 *)
+  0xca100084;       (* arm_EOR X4 X4 X16 *)
+  0xda100084;       (* arm_SBC X4 X4 X16 *)
+  0xca0000a5;       (* arm_EOR X5 X5 X0 *)
+  0xeb0000a5;       (* arm_SUBS X5 X5 X0 *)
+  0xca0000c6;       (* arm_EOR X6 X6 X0 *)
+  0xda0000c6;       (* arm_SBC X6 X6 X0 *)
+  0xca100010;       (* arm_EOR X16 X0 X16 *)
+  0xab09016b;       (* arm_ADDS X11 X11 X9 *)
+  0xba0a018c;       (* arm_ADCS X12 X12 X10 *)
+  0xba1f01ad;       (* arm_ADCS X13 X13 XZR *)
+  0x9a1f01ce;       (* arm_ADC X14 X14 XZR *)
+  0x9b057c62;       (* arm_MUL X2 X3 X5 *)
+  0x9bc57c60;       (* arm_UMULH X0 X3 X5 *)
+  0x9b067c8f;       (* arm_MUL X15 X4 X6 *)
+  0x9bc67c81;       (* arm_UMULH X1 X4 X6 *)
+  0xeb030084;       (* arm_SUBS X4 X4 X3 *)
+  0xda842484;       (* arm_CNEG X4 X4 Condition_CC *)
+  0xda9f23e9;       (* arm_CSETM X9 Condition_CC *)
+  0xab0001ef;       (* arm_ADDS X15 X15 X0 *)
+  0x9a1f0021;       (* arm_ADC X1 X1 XZR *)
+  0xeb0600a6;       (* arm_SUBS X6 X5 X6 *)
+  0xda8624c6;       (* arm_CNEG X6 X6 Condition_CC *)
+  0xda892129;       (* arm_CINV X9 X9 Condition_CC *)
+  0x9b067c85;       (* arm_MUL X5 X4 X6 *)
+  0x9bc67c86;       (* arm_UMULH X6 X4 X6 *)
+  0xab0f0040;       (* arm_ADDS X0 X2 X15 *)
+  0xba0101ef;       (* arm_ADCS X15 X15 X1 *)
+  0x9a1f0021;       (* arm_ADC X1 X1 XZR *)
+  0xb100053f;       (* arm_CMN X9 (rvalue (word 1)) *)
+  0xca0900a5;       (* arm_EOR X5 X5 X9 *)
+  0xba0000a0;       (* arm_ADCS X0 X5 X0 *)
+  0xca0900c6;       (* arm_EOR X6 X6 X9 *)
+  0xba0f00cf;       (* arm_ADCS X15 X6 X15 *)
+  0x9a090021;       (* arm_ADC X1 X1 X9 *)
+  0xab070169;       (* arm_ADDS X9 X11 X7 *)
+  0xba08018a;       (* arm_ADCS X10 X12 X8 *)
+  0xba0b01ab;       (* arm_ADCS X11 X13 X11 *)
+  0xba0c01cc;       (* arm_ADCS X12 X14 X12 *)
+  0xba1f01ad;       (* arm_ADCS X13 X13 XZR *)
+  0x9a1f01ce;       (* arm_ADC X14 X14 XZR *)
+  0xb100061f;       (* arm_CMN X16 (rvalue (word 1)) *)
+  0xca100042;       (* arm_EOR X2 X2 X16 *)
+  0xba090049;       (* arm_ADCS X9 X2 X9 *)
+  0xca100000;       (* arm_EOR X0 X0 X16 *)
+  0xba0a000a;       (* arm_ADCS X10 X0 X10 *)
+  0xca1001ef;       (* arm_EOR X15 X15 X16 *)
+  0xba0b01eb;       (* arm_ADCS X11 X15 X11 *)
+  0xca100021;       (* arm_EOR X1 X1 X16 *)
+  0xba0c002c;       (* arm_ADCS X12 X1 X12 *)
+  0xba1001ad;       (* arm_ADCS X13 X13 X16 *)
+  0x9a1001ce;       (* arm_ADC X14 X14 X16 *)
+  0xd28004c3;       (* arm_MOV X3 (rvalue (word 38)) *)
+  0x92407d65;       (* arm_AND X5 X11 (rvalue (word 4294967295)) *)
+  0xd360fd64;       (* arm_LSR X4 X11 32 *)
+  0x9b057c65;       (* arm_MUL X5 X3 X5 *)
+  0x9b047c64;       (* arm_MUL X4 X3 X4 *)
+  0xab0500e7;       (* arm_ADDS X7 X7 X5 *)
+  0x92407d85;       (* arm_AND X5 X12 (rvalue (word 4294967295)) *)
+  0xd360fd8c;       (* arm_LSR X12 X12 32 *)
+  0x9b057c65;       (* arm_MUL X5 X3 X5 *)
+  0x9b0c7c6c;       (* arm_MUL X12 X3 X12 *)
+  0xba050108;       (* arm_ADCS X8 X8 X5 *)
+  0x92407da5;       (* arm_AND X5 X13 (rvalue (word 4294967295)) *)
+  0xd360fdad;       (* arm_LSR X13 X13 32 *)
+  0x9b057c65;       (* arm_MUL X5 X3 X5 *)
+  0x9b0d7c6d;       (* arm_MUL X13 X3 X13 *)
+  0xba050129;       (* arm_ADCS X9 X9 X5 *)
+  0x92407dc5;       (* arm_AND X5 X14 (rvalue (word 4294967295)) *)
+  0xd360fdce;       (* arm_LSR X14 X14 32 *)
+  0x9b057c65;       (* arm_MUL X5 X3 X5 *)
+  0x9b0e7c6e;       (* arm_MUL X14 X3 X14 *)
+  0xba05014a;       (* arm_ADCS X10 X10 X5 *)
+  0x9a9f37eb;       (* arm_CSET X11 Condition_CS *)
+  0xd3607c85;       (* arm_LSL X5 X4 32 *)
+  0xab0500e7;       (* arm_ADDS X7 X7 X5 *)
+  0x93c48185;       (* arm_EXTR X5 X12 X4 32 *)
+  0xba050108;       (* arm_ADCS X8 X8 X5 *)
+  0x93cc81a5;       (* arm_EXTR X5 X13 X12 32 *)
+  0xba050129;       (* arm_ADCS X9 X9 X5 *)
+  0x93cd81c5;       (* arm_EXTR X5 X14 X13 32 *)
+  0xba05014a;       (* arm_ADCS X10 X10 X5 *)
+  0xd360fdc5;       (* arm_LSR X5 X14 32 *)
+  0x9a05016b;       (* arm_ADC X11 X11 X5 *)
+  0xab0a015f;       (* arm_CMN X10 X10 *)
+  0x9240f94a;       (* arm_AND X10 X10 (rvalue (word 9223372036854775807)) *)
+  0x9a0b0160;       (* arm_ADC X0 X11 X11 *)
+  0xd2800263;       (* arm_MOV X3 (rvalue (word 19)) *)
+  0x9b007c65;       (* arm_MUL X5 X3 X0 *)
+  0xab0500e7;       (* arm_ADDS X7 X7 X5 *)
+  0xba1f0108;       (* arm_ADCS X8 X8 XZR *)
+  0xba1f0129;       (* arm_ADCS X9 X9 XZR *)
+  0x9a1f014a;       (* arm_ADC X10 X10 XZR *)
+  0xa90823e7;       (* arm_STP X7 X8 SP (Immediate_Offset (iword (&128))) *)
+  0xa9092be9;       (* arm_STP X9 X10 SP (Immediate_Offset (iword (&144))) *)
+  0xa9461be5;       (* arm_LDP X5 X6 SP (Immediate_Offset (iword (&96))) *)
   0xa9420fe4;       (* arm_LDP X4 X3 SP (Immediate_Offset (iword (&32))) *)
   0xeb0400a5;       (* arm_SUBS X5 X5 X4 *)
   0xfa0300c6;       (* arm_SBCS X6 X6 X3 *)
-  0xa94523e7;       (* arm_LDP X7 X8 SP (Immediate_Offset (iword (&80))) *)
+  0xa94723e7;       (* arm_LDP X7 X8 SP (Immediate_Offset (iword (&112))) *)
   0xa9430fe4;       (* arm_LDP X4 X3 SP (Immediate_Offset (iword (&48))) *)
   0xfa0400e7;       (* arm_SBCS X7 X7 X4 *)
   0xfa030108;       (* arm_SBCS X8 X8 X3 *)
@@ -575,13 +897,13 @@ let edwards25519_pepadd_mc = define_assert_from_elf
   0xfa1f00c6;       (* arm_SBCS X6 X6 XZR *)
   0xfa1f00e7;       (* arm_SBCS X7 X7 XZR *)
   0xda1f0108;       (* arm_SBC X8 X8 XZR *)
-  0xa90a1be5;       (* arm_STP X5 X6 SP (Immediate_Offset (iword (&160))) *)
-  0xa90b23e7;       (* arm_STP X7 X8 SP (Immediate_Offset (iword (&176))) *)
-  0xa94413e3;       (* arm_LDP X3 X4 SP (Immediate_Offset (iword (&64))) *)
+  0xa9001be5;       (* arm_STP X5 X6 SP (Immediate_Offset (iword (&0))) *)
+  0xa90123e7;       (* arm_STP X7 X8 SP (Immediate_Offset (iword (&16))) *)
+  0xa94613e3;       (* arm_LDP X3 X4 SP (Immediate_Offset (iword (&96))) *)
   0xa94223e7;       (* arm_LDP X7 X8 SP (Immediate_Offset (iword (&32))) *)
   0xab070063;       (* arm_ADDS X3 X3 X7 *)
   0xba080084;       (* arm_ADCS X4 X4 X8 *)
-  0xa9451be5;       (* arm_LDP X5 X6 SP (Immediate_Offset (iword (&80))) *)
+  0xa9471be5;       (* arm_LDP X5 X6 SP (Immediate_Offset (iword (&112))) *)
   0xa94323e7;       (* arm_LDP X7 X8 SP (Immediate_Offset (iword (&48))) *)
   0xba0700a5;       (* arm_ADCS X5 X5 X7 *)
   0xba0800c6;       (* arm_ADCS X6 X6 X8 *)
@@ -591,171 +913,42 @@ let edwards25519_pepadd_mc = define_assert_from_elf
   0xba1f0084;       (* arm_ADCS X4 X4 XZR *)
   0xba1f00a5;       (* arm_ADCS X5 X5 XZR *)
   0x9a1f00c6;       (* arm_ADC X6 X6 XZR *)
-  0xa90213e3;       (* arm_STP X3 X4 SP (Immediate_Offset (iword (&32))) *)
-  0xa9031be5;       (* arm_STP X5 X6 SP (Immediate_Offset (iword (&48))) *)
-  0xa94813e3;       (* arm_LDP X3 X4 SP (Immediate_Offset (iword (&128))) *)
-  0xa9401be5;       (* arm_LDP X5 X6 SP (Immediate_Offset (iword (&0))) *)
-  0x9b057c67;       (* arm_MUL X7 X3 X5 *)
-  0x9bc57c68;       (* arm_UMULH X8 X3 X5 *)
-  0x9b067c89;       (* arm_MUL X9 X4 X6 *)
-  0x9bc67c8a;       (* arm_UMULH X10 X4 X6 *)
-  0xeb030084;       (* arm_SUBS X4 X4 X3 *)
-  0xda842484;       (* arm_CNEG X4 X4 Condition_CC *)
-  0xda9f23f0;       (* arm_CSETM X16 Condition_CC *)
-  0xab080129;       (* arm_ADDS X9 X9 X8 *)
-  0x9a1f014a;       (* arm_ADC X10 X10 XZR *)
-  0xeb0600a3;       (* arm_SUBS X3 X5 X6 *)
-  0xda832463;       (* arm_CNEG X3 X3 Condition_CC *)
-  0xda902210;       (* arm_CINV X16 X16 Condition_CC *)
-  0x9b037c8f;       (* arm_MUL X15 X4 X3 *)
-  0x9bc37c83;       (* arm_UMULH X3 X4 X3 *)
-  0xab0900e8;       (* arm_ADDS X8 X7 X9 *)
-  0xba0a0129;       (* arm_ADCS X9 X9 X10 *)
-  0x9a1f014a;       (* arm_ADC X10 X10 XZR *)
-  0xb100061f;       (* arm_CMN X16 (rvalue (word 1)) *)
-  0xca1001ef;       (* arm_EOR X15 X15 X16 *)
-  0xba0801e8;       (* arm_ADCS X8 X15 X8 *)
-  0xca100063;       (* arm_EOR X3 X3 X16 *)
-  0xba090069;       (* arm_ADCS X9 X3 X9 *)
-  0x9a10014a;       (* arm_ADC X10 X10 X16 *)
-  0xa94913e3;       (* arm_LDP X3 X4 SP (Immediate_Offset (iword (&144))) *)
-  0xa9411be5;       (* arm_LDP X5 X6 SP (Immediate_Offset (iword (&16))) *)
-  0x9b057c6b;       (* arm_MUL X11 X3 X5 *)
-  0x9bc57c6c;       (* arm_UMULH X12 X3 X5 *)
-  0x9b067c8d;       (* arm_MUL X13 X4 X6 *)
-  0x9bc67c8e;       (* arm_UMULH X14 X4 X6 *)
-  0xeb030084;       (* arm_SUBS X4 X4 X3 *)
-  0xda842484;       (* arm_CNEG X4 X4 Condition_CC *)
-  0xda9f23f0;       (* arm_CSETM X16 Condition_CC *)
-  0xab0c01ad;       (* arm_ADDS X13 X13 X12 *)
-  0x9a1f01ce;       (* arm_ADC X14 X14 XZR *)
-  0xeb0600a3;       (* arm_SUBS X3 X5 X6 *)
-  0xda832463;       (* arm_CNEG X3 X3 Condition_CC *)
-  0xda902210;       (* arm_CINV X16 X16 Condition_CC *)
-  0x9b037c8f;       (* arm_MUL X15 X4 X3 *)
-  0x9bc37c83;       (* arm_UMULH X3 X4 X3 *)
-  0xab0d016c;       (* arm_ADDS X12 X11 X13 *)
-  0xba0e01ad;       (* arm_ADCS X13 X13 X14 *)
-  0x9a1f01ce;       (* arm_ADC X14 X14 XZR *)
-  0xb100061f;       (* arm_CMN X16 (rvalue (word 1)) *)
-  0xca1001ef;       (* arm_EOR X15 X15 X16 *)
-  0xba0c01ec;       (* arm_ADCS X12 X15 X12 *)
-  0xca100063;       (* arm_EOR X3 X3 X16 *)
-  0xba0d006d;       (* arm_ADCS X13 X3 X13 *)
-  0x9a1001ce;       (* arm_ADC X14 X14 X16 *)
-  0xa94913e3;       (* arm_LDP X3 X4 SP (Immediate_Offset (iword (&144))) *)
-  0xa94843ef;       (* arm_LDP X15 X16 SP (Immediate_Offset (iword (&128))) *)
-  0xeb0f0063;       (* arm_SUBS X3 X3 X15 *)
-  0xfa100084;       (* arm_SBCS X4 X4 X16 *)
-  0xda9f23f0;       (* arm_CSETM X16 Condition_CC *)
-  0xa94003ef;       (* arm_LDP X15 X0 SP (Immediate_Offset (iword (&0))) *)
-  0xeb0501e5;       (* arm_SUBS X5 X15 X5 *)
-  0xfa060006;       (* arm_SBCS X6 X0 X6 *)
-  0xda9f23e0;       (* arm_CSETM X0 Condition_CC *)
-  0xca100063;       (* arm_EOR X3 X3 X16 *)
-  0xeb100063;       (* arm_SUBS X3 X3 X16 *)
-  0xca100084;       (* arm_EOR X4 X4 X16 *)
-  0xda100084;       (* arm_SBC X4 X4 X16 *)
-  0xca0000a5;       (* arm_EOR X5 X5 X0 *)
-  0xeb0000a5;       (* arm_SUBS X5 X5 X0 *)
-  0xca0000c6;       (* arm_EOR X6 X6 X0 *)
-  0xda0000c6;       (* arm_SBC X6 X6 X0 *)
-  0xca100010;       (* arm_EOR X16 X0 X16 *)
-  0xab09016b;       (* arm_ADDS X11 X11 X9 *)
-  0xba0a018c;       (* arm_ADCS X12 X12 X10 *)
-  0xba1f01ad;       (* arm_ADCS X13 X13 XZR *)
-  0x9a1f01ce;       (* arm_ADC X14 X14 XZR *)
-  0x9b057c62;       (* arm_MUL X2 X3 X5 *)
-  0x9bc57c60;       (* arm_UMULH X0 X3 X5 *)
-  0x9b067c8f;       (* arm_MUL X15 X4 X6 *)
-  0x9bc67c81;       (* arm_UMULH X1 X4 X6 *)
-  0xeb030084;       (* arm_SUBS X4 X4 X3 *)
-  0xda842484;       (* arm_CNEG X4 X4 Condition_CC *)
-  0xda9f23e9;       (* arm_CSETM X9 Condition_CC *)
-  0xab0001ef;       (* arm_ADDS X15 X15 X0 *)
-  0x9a1f0021;       (* arm_ADC X1 X1 XZR *)
-  0xeb0600a6;       (* arm_SUBS X6 X5 X6 *)
-  0xda8624c6;       (* arm_CNEG X6 X6 Condition_CC *)
-  0xda892129;       (* arm_CINV X9 X9 Condition_CC *)
-  0x9b067c85;       (* arm_MUL X5 X4 X6 *)
-  0x9bc67c86;       (* arm_UMULH X6 X4 X6 *)
-  0xab0f0040;       (* arm_ADDS X0 X2 X15 *)
-  0xba0101ef;       (* arm_ADCS X15 X15 X1 *)
-  0x9a1f0021;       (* arm_ADC X1 X1 XZR *)
-  0xb100053f;       (* arm_CMN X9 (rvalue (word 1)) *)
-  0xca0900a5;       (* arm_EOR X5 X5 X9 *)
-  0xba0000a0;       (* arm_ADCS X0 X5 X0 *)
-  0xca0900c6;       (* arm_EOR X6 X6 X9 *)
-  0xba0f00cf;       (* arm_ADCS X15 X6 X15 *)
-  0x9a090021;       (* arm_ADC X1 X1 X9 *)
-  0xab070169;       (* arm_ADDS X9 X11 X7 *)
-  0xba08018a;       (* arm_ADCS X10 X12 X8 *)
-  0xba0b01ab;       (* arm_ADCS X11 X13 X11 *)
-  0xba0c01cc;       (* arm_ADCS X12 X14 X12 *)
-  0xba1f01ad;       (* arm_ADCS X13 X13 XZR *)
-  0x9a1f01ce;       (* arm_ADC X14 X14 XZR *)
-  0xb100061f;       (* arm_CMN X16 (rvalue (word 1)) *)
-  0xca100042;       (* arm_EOR X2 X2 X16 *)
-  0xba090049;       (* arm_ADCS X9 X2 X9 *)
-  0xca100000;       (* arm_EOR X0 X0 X16 *)
-  0xba0a000a;       (* arm_ADCS X10 X0 X10 *)
-  0xca1001ef;       (* arm_EOR X15 X15 X16 *)
-  0xba0b01eb;       (* arm_ADCS X11 X15 X11 *)
-  0xca100021;       (* arm_EOR X1 X1 X16 *)
-  0xba0c002c;       (* arm_ADCS X12 X1 X12 *)
-  0xba1001ad;       (* arm_ADCS X13 X13 X16 *)
-  0x9a1001ce;       (* arm_ADC X14 X14 X16 *)
-  0xd28004c3;       (* arm_MOV X3 (rvalue (word 38)) *)
-  0x92407d65;       (* arm_AND X5 X11 (rvalue (word 4294967295)) *)
-  0xd360fd64;       (* arm_LSR X4 X11 32 *)
-  0x9b057c65;       (* arm_MUL X5 X3 X5 *)
-  0x9b047c64;       (* arm_MUL X4 X3 X4 *)
-  0xab0500e7;       (* arm_ADDS X7 X7 X5 *)
-  0x92407d85;       (* arm_AND X5 X12 (rvalue (word 4294967295)) *)
-  0xd360fd8c;       (* arm_LSR X12 X12 32 *)
-  0x9b057c65;       (* arm_MUL X5 X3 X5 *)
-  0x9b0c7c6c;       (* arm_MUL X12 X3 X12 *)
-  0xba050108;       (* arm_ADCS X8 X8 X5 *)
-  0x92407da5;       (* arm_AND X5 X13 (rvalue (word 4294967295)) *)
-  0xd360fdad;       (* arm_LSR X13 X13 32 *)
-  0x9b057c65;       (* arm_MUL X5 X3 X5 *)
-  0x9b0d7c6d;       (* arm_MUL X13 X3 X13 *)
-  0xba050129;       (* arm_ADCS X9 X9 X5 *)
-  0x92407dc5;       (* arm_AND X5 X14 (rvalue (word 4294967295)) *)
-  0xd360fdce;       (* arm_LSR X14 X14 32 *)
-  0x9b057c65;       (* arm_MUL X5 X3 X5 *)
-  0x9b0e7c6e;       (* arm_MUL X14 X3 X14 *)
-  0xba05014a;       (* arm_ADCS X10 X10 X5 *)
-  0x9a9f37eb;       (* arm_CSET X11 Condition_CS *)
-  0xd3607c85;       (* arm_LSL X5 X4 32 *)
-  0xab0500e7;       (* arm_ADDS X7 X7 X5 *)
-  0x93c48185;       (* arm_EXTR X5 X12 X4 32 *)
-  0xba050108;       (* arm_ADCS X8 X8 X5 *)
-  0x93cc81a5;       (* arm_EXTR X5 X13 X12 32 *)
-  0xba050129;       (* arm_ADCS X9 X9 X5 *)
-  0x93cd81c5;       (* arm_EXTR X5 X14 X13 32 *)
-  0xba05014a;       (* arm_ADCS X10 X10 X5 *)
-  0xd360fdc5;       (* arm_LSR X5 X14 32 *)
-  0x9a05016b;       (* arm_ADC X11 X11 X5 *)
-  0xab0a015f;       (* arm_CMN X10 X10 *)
-  0xb241014a;       (* arm_ORR X10 X10 (rvalue (word 9223372036854775808)) *)
-  0x9a0b0160;       (* arm_ADC X0 X11 X11 *)
-  0xd2800263;       (* arm_MOV X3 (rvalue (word 19)) *)
-  0x9b000c65;       (* arm_MADD X5 X3 X0 X3 *)
-  0xab0500e7;       (* arm_ADDS X7 X7 X5 *)
-  0xba1f0108;       (* arm_ADCS X8 X8 XZR *)
-  0xba1f0129;       (* arm_ADCS X9 X9 XZR *)
-  0xba1f014a;       (* arm_ADCS X10 X10 XZR *)
-  0x9a9f3063;       (* arm_CSEL X3 X3 XZR Condition_CC *)
-  0xeb0300e7;       (* arm_SUBS X7 X7 X3 *)
-  0xfa1f0108;       (* arm_SBCS X8 X8 XZR *)
-  0xfa1f0129;       (* arm_SBCS X9 X9 XZR *)
-  0xda1f014a;       (* arm_SBC X10 X10 XZR *)
-  0x9240f94a;       (* arm_AND X10 X10 (rvalue (word 9223372036854775807)) *)
-  0xa9042227;       (* arm_STP X7 X8 X17 (Immediate_Offset (iword (&64))) *)
-  0xa9052a29;       (* arm_STP X9 X10 X17 (Immediate_Offset (iword (&80))) *)
-  0xa94a13e3;       (* arm_LDP X3 X4 SP (Immediate_Offset (iword (&160))) *)
+  0xa90a13e3;       (* arm_STP X3 X4 SP (Immediate_Offset (iword (&160))) *)
+  0xa90b1be5;       (* arm_STP X5 X6 SP (Immediate_Offset (iword (&176))) *)
   0xa9481be5;       (* arm_LDP X5 X6 SP (Immediate_Offset (iword (&128))) *)
+  0xa9440fe4;       (* arm_LDP X4 X3 SP (Immediate_Offset (iword (&64))) *)
+  0xeb0400a5;       (* arm_SUBS X5 X5 X4 *)
+  0xfa0300c6;       (* arm_SBCS X6 X6 X3 *)
+  0xa94923e7;       (* arm_LDP X7 X8 SP (Immediate_Offset (iword (&144))) *)
+  0xa9450fe4;       (* arm_LDP X4 X3 SP (Immediate_Offset (iword (&80))) *)
+  0xfa0400e7;       (* arm_SBCS X7 X7 X4 *)
+  0xfa030108;       (* arm_SBCS X8 X8 X3 *)
+  0xd28004c4;       (* arm_MOV X4 (rvalue (word 38)) *)
+  0x9a9f3083;       (* arm_CSEL X3 X4 XZR Condition_CC *)
+  0xeb0300a5;       (* arm_SUBS X5 X5 X3 *)
+  0xfa1f00c6;       (* arm_SBCS X6 X6 XZR *)
+  0xfa1f00e7;       (* arm_SBCS X7 X7 XZR *)
+  0xda1f0108;       (* arm_SBC X8 X8 XZR *)
+  0xa9021be5;       (* arm_STP X5 X6 SP (Immediate_Offset (iword (&32))) *)
+  0xa90323e7;       (* arm_STP X7 X8 SP (Immediate_Offset (iword (&48))) *)
+  0xa94813e3;       (* arm_LDP X3 X4 SP (Immediate_Offset (iword (&128))) *)
+  0xa94423e7;       (* arm_LDP X7 X8 SP (Immediate_Offset (iword (&64))) *)
+  0xab070063;       (* arm_ADDS X3 X3 X7 *)
+  0xba080084;       (* arm_ADCS X4 X4 X8 *)
+  0xa9491be5;       (* arm_LDP X5 X6 SP (Immediate_Offset (iword (&144))) *)
+  0xa94523e7;       (* arm_LDP X7 X8 SP (Immediate_Offset (iword (&80))) *)
+  0xba0700a5;       (* arm_ADCS X5 X5 X7 *)
+  0xba0800c6;       (* arm_ADCS X6 X6 X8 *)
+  0xd28004c9;       (* arm_MOV X9 (rvalue (word 38)) *)
+  0x9a9f2129;       (* arm_CSEL X9 X9 XZR Condition_CS *)
+  0xab090063;       (* arm_ADDS X3 X3 X9 *)
+  0xba1f0084;       (* arm_ADCS X4 X4 XZR *)
+  0xba1f00a5;       (* arm_ADCS X5 X5 XZR *)
+  0x9a1f00c6;       (* arm_ADC X6 X6 XZR *)
+  0xa90613e3;       (* arm_STP X3 X4 SP (Immediate_Offset (iword (&96))) *)
+  0xa9071be5;       (* arm_STP X5 X6 SP (Immediate_Offset (iword (&112))) *)
+  0xa94013e3;       (* arm_LDP X3 X4 SP (Immediate_Offset (iword (&0))) *)
+  0xa94a1be5;       (* arm_LDP X5 X6 SP (Immediate_Offset (iword (&160))) *)
   0x9b057c67;       (* arm_MUL X7 X3 X5 *)
   0x9bc57c68;       (* arm_UMULH X8 X3 X5 *)
   0x9b067c89;       (* arm_MUL X9 X4 X6 *)
@@ -779,8 +972,8 @@ let edwards25519_pepadd_mc = define_assert_from_elf
   0xca100063;       (* arm_EOR X3 X3 X16 *)
   0xba090069;       (* arm_ADCS X9 X3 X9 *)
   0x9a10014a;       (* arm_ADC X10 X10 X16 *)
-  0xa94b13e3;       (* arm_LDP X3 X4 SP (Immediate_Offset (iword (&176))) *)
-  0xa9491be5;       (* arm_LDP X5 X6 SP (Immediate_Offset (iword (&144))) *)
+  0xa94113e3;       (* arm_LDP X3 X4 SP (Immediate_Offset (iword (&16))) *)
+  0xa94b1be5;       (* arm_LDP X5 X6 SP (Immediate_Offset (iword (&176))) *)
   0x9b057c6b;       (* arm_MUL X11 X3 X5 *)
   0x9bc57c6c;       (* arm_UMULH X12 X3 X5 *)
   0x9b067c8d;       (* arm_MUL X13 X4 X6 *)
@@ -804,12 +997,12 @@ let edwards25519_pepadd_mc = define_assert_from_elf
   0xca100063;       (* arm_EOR X3 X3 X16 *)
   0xba0d006d;       (* arm_ADCS X13 X3 X13 *)
   0x9a1001ce;       (* arm_ADC X14 X14 X16 *)
-  0xa94b13e3;       (* arm_LDP X3 X4 SP (Immediate_Offset (iword (&176))) *)
-  0xa94a43ef;       (* arm_LDP X15 X16 SP (Immediate_Offset (iword (&160))) *)
+  0xa94113e3;       (* arm_LDP X3 X4 SP (Immediate_Offset (iword (&16))) *)
+  0xa94043ef;       (* arm_LDP X15 X16 SP (Immediate_Offset (iword (&0))) *)
   0xeb0f0063;       (* arm_SUBS X3 X3 X15 *)
   0xfa100084;       (* arm_SBCS X4 X4 X16 *)
   0xda9f23f0;       (* arm_CSETM X16 Condition_CC *)
-  0xa94803ef;       (* arm_LDP X15 X0 SP (Immediate_Offset (iword (&128))) *)
+  0xa94a03ef;       (* arm_LDP X15 X0 SP (Immediate_Offset (iword (&160))) *)
   0xeb0501e5;       (* arm_SUBS X5 X15 X5 *)
   0xfa060006;       (* arm_SBCS X6 X0 X6 *)
   0xda9f23e0;       (* arm_CSETM X0 Condition_CC *)
@@ -913,8 +1106,8 @@ let edwards25519_pepadd_mc = define_assert_from_elf
   0xfa1f0129;       (* arm_SBCS X9 X9 XZR *)
   0xda1f014a;       (* arm_SBC X10 X10 XZR *)
   0x9240f94a;       (* arm_AND X10 X10 (rvalue (word 9223372036854775807)) *)
-  0xa9002227;       (* arm_STP X7 X8 X17 (Immediate_Offset (iword (&0))) *)
-  0xa9012a29;       (* arm_STP X9 X10 X17 (Immediate_Offset (iword (&16))) *)
+  0xa9062227;       (* arm_STP X7 X8 X17 (Immediate_Offset (iword (&96))) *)
+  0xa9072a29;       (* arm_STP X9 X10 X17 (Immediate_Offset (iword (&112))) *)
   0xa94013e3;       (* arm_LDP X3 X4 SP (Immediate_Offset (iword (&0))) *)
   0xa9421be5;       (* arm_LDP X5 X6 SP (Immediate_Offset (iword (&32))) *)
   0x9b057c67;       (* arm_MUL X7 X3 X5 *)
@@ -1074,10 +1267,10 @@ let edwards25519_pepadd_mc = define_assert_from_elf
   0xfa1f0129;       (* arm_SBCS X9 X9 XZR *)
   0xda1f014a;       (* arm_SBC X10 X10 XZR *)
   0x9240f94a;       (* arm_AND X10 X10 (rvalue (word 9223372036854775807)) *)
-  0xa9022227;       (* arm_STP X7 X8 X17 (Immediate_Offset (iword (&32))) *)
-  0xa9032a29;       (* arm_STP X9 X10 X17 (Immediate_Offset (iword (&48))) *)
-  0xa94a13e3;       (* arm_LDP X3 X4 SP (Immediate_Offset (iword (&160))) *)
-  0xa9421be5;       (* arm_LDP X5 X6 SP (Immediate_Offset (iword (&32))) *)
+  0xa9002227;       (* arm_STP X7 X8 X17 (Immediate_Offset (iword (&0))) *)
+  0xa9012a29;       (* arm_STP X9 X10 X17 (Immediate_Offset (iword (&16))) *)
+  0xa94613e3;       (* arm_LDP X3 X4 SP (Immediate_Offset (iword (&96))) *)
+  0xa94a1be5;       (* arm_LDP X5 X6 SP (Immediate_Offset (iword (&160))) *)
   0x9b057c67;       (* arm_MUL X7 X3 X5 *)
   0x9bc57c68;       (* arm_UMULH X8 X3 X5 *)
   0x9b067c89;       (* arm_MUL X9 X4 X6 *)
@@ -1101,8 +1294,8 @@ let edwards25519_pepadd_mc = define_assert_from_elf
   0xca100063;       (* arm_EOR X3 X3 X16 *)
   0xba090069;       (* arm_ADCS X9 X3 X9 *)
   0x9a10014a;       (* arm_ADC X10 X10 X16 *)
-  0xa94b13e3;       (* arm_LDP X3 X4 SP (Immediate_Offset (iword (&176))) *)
-  0xa9431be5;       (* arm_LDP X5 X6 SP (Immediate_Offset (iword (&48))) *)
+  0xa94713e3;       (* arm_LDP X3 X4 SP (Immediate_Offset (iword (&112))) *)
+  0xa94b1be5;       (* arm_LDP X5 X6 SP (Immediate_Offset (iword (&176))) *)
   0x9b057c6b;       (* arm_MUL X11 X3 X5 *)
   0x9bc57c6c;       (* arm_UMULH X12 X3 X5 *)
   0x9b067c8d;       (* arm_MUL X13 X4 X6 *)
@@ -1126,12 +1319,12 @@ let edwards25519_pepadd_mc = define_assert_from_elf
   0xca100063;       (* arm_EOR X3 X3 X16 *)
   0xba0d006d;       (* arm_ADCS X13 X3 X13 *)
   0x9a1001ce;       (* arm_ADC X14 X14 X16 *)
-  0xa94b13e3;       (* arm_LDP X3 X4 SP (Immediate_Offset (iword (&176))) *)
-  0xa94a43ef;       (* arm_LDP X15 X16 SP (Immediate_Offset (iword (&160))) *)
+  0xa94713e3;       (* arm_LDP X3 X4 SP (Immediate_Offset (iword (&112))) *)
+  0xa94643ef;       (* arm_LDP X15 X16 SP (Immediate_Offset (iword (&96))) *)
   0xeb0f0063;       (* arm_SUBS X3 X3 X15 *)
   0xfa100084;       (* arm_SBCS X4 X4 X16 *)
   0xda9f23f0;       (* arm_CSETM X16 Condition_CC *)
-  0xa94203ef;       (* arm_LDP X15 X0 SP (Immediate_Offset (iword (&32))) *)
+  0xa94a03ef;       (* arm_LDP X15 X0 SP (Immediate_Offset (iword (&160))) *)
   0xeb0501e5;       (* arm_SUBS X5 X15 X5 *)
   0xfa060006;       (* arm_SBCS X6 X0 X6 *)
   0xda9f23e0;       (* arm_CSETM X0 Condition_CC *)
@@ -1235,14 +1428,175 @@ let edwards25519_pepadd_mc = define_assert_from_elf
   0xfa1f0129;       (* arm_SBCS X9 X9 XZR *)
   0xda1f014a;       (* arm_SBC X10 X10 XZR *)
   0x9240f94a;       (* arm_AND X10 X10 (rvalue (word 9223372036854775807)) *)
-  0xa9062227;       (* arm_STP X7 X8 X17 (Immediate_Offset (iword (&96))) *)
-  0xa9072a29;       (* arm_STP X9 X10 X17 (Immediate_Offset (iword (&112))) *)
+  0xa9022227;       (* arm_STP X7 X8 X17 (Immediate_Offset (iword (&32))) *)
+  0xa9032a29;       (* arm_STP X9 X10 X17 (Immediate_Offset (iword (&48))) *)
+  0xa94213e3;       (* arm_LDP X3 X4 SP (Immediate_Offset (iword (&32))) *)
+  0xa9461be5;       (* arm_LDP X5 X6 SP (Immediate_Offset (iword (&96))) *)
+  0x9b057c67;       (* arm_MUL X7 X3 X5 *)
+  0x9bc57c68;       (* arm_UMULH X8 X3 X5 *)
+  0x9b067c89;       (* arm_MUL X9 X4 X6 *)
+  0x9bc67c8a;       (* arm_UMULH X10 X4 X6 *)
+  0xeb030084;       (* arm_SUBS X4 X4 X3 *)
+  0xda842484;       (* arm_CNEG X4 X4 Condition_CC *)
+  0xda9f23f0;       (* arm_CSETM X16 Condition_CC *)
+  0xab080129;       (* arm_ADDS X9 X9 X8 *)
+  0x9a1f014a;       (* arm_ADC X10 X10 XZR *)
+  0xeb0600a3;       (* arm_SUBS X3 X5 X6 *)
+  0xda832463;       (* arm_CNEG X3 X3 Condition_CC *)
+  0xda902210;       (* arm_CINV X16 X16 Condition_CC *)
+  0x9b037c8f;       (* arm_MUL X15 X4 X3 *)
+  0x9bc37c83;       (* arm_UMULH X3 X4 X3 *)
+  0xab0900e8;       (* arm_ADDS X8 X7 X9 *)
+  0xba0a0129;       (* arm_ADCS X9 X9 X10 *)
+  0x9a1f014a;       (* arm_ADC X10 X10 XZR *)
+  0xb100061f;       (* arm_CMN X16 (rvalue (word 1)) *)
+  0xca1001ef;       (* arm_EOR X15 X15 X16 *)
+  0xba0801e8;       (* arm_ADCS X8 X15 X8 *)
+  0xca100063;       (* arm_EOR X3 X3 X16 *)
+  0xba090069;       (* arm_ADCS X9 X3 X9 *)
+  0x9a10014a;       (* arm_ADC X10 X10 X16 *)
+  0xa94313e3;       (* arm_LDP X3 X4 SP (Immediate_Offset (iword (&48))) *)
+  0xa9471be5;       (* arm_LDP X5 X6 SP (Immediate_Offset (iword (&112))) *)
+  0x9b057c6b;       (* arm_MUL X11 X3 X5 *)
+  0x9bc57c6c;       (* arm_UMULH X12 X3 X5 *)
+  0x9b067c8d;       (* arm_MUL X13 X4 X6 *)
+  0x9bc67c8e;       (* arm_UMULH X14 X4 X6 *)
+  0xeb030084;       (* arm_SUBS X4 X4 X3 *)
+  0xda842484;       (* arm_CNEG X4 X4 Condition_CC *)
+  0xda9f23f0;       (* arm_CSETM X16 Condition_CC *)
+  0xab0c01ad;       (* arm_ADDS X13 X13 X12 *)
+  0x9a1f01ce;       (* arm_ADC X14 X14 XZR *)
+  0xeb0600a3;       (* arm_SUBS X3 X5 X6 *)
+  0xda832463;       (* arm_CNEG X3 X3 Condition_CC *)
+  0xda902210;       (* arm_CINV X16 X16 Condition_CC *)
+  0x9b037c8f;       (* arm_MUL X15 X4 X3 *)
+  0x9bc37c83;       (* arm_UMULH X3 X4 X3 *)
+  0xab0d016c;       (* arm_ADDS X12 X11 X13 *)
+  0xba0e01ad;       (* arm_ADCS X13 X13 X14 *)
+  0x9a1f01ce;       (* arm_ADC X14 X14 XZR *)
+  0xb100061f;       (* arm_CMN X16 (rvalue (word 1)) *)
+  0xca1001ef;       (* arm_EOR X15 X15 X16 *)
+  0xba0c01ec;       (* arm_ADCS X12 X15 X12 *)
+  0xca100063;       (* arm_EOR X3 X3 X16 *)
+  0xba0d006d;       (* arm_ADCS X13 X3 X13 *)
+  0x9a1001ce;       (* arm_ADC X14 X14 X16 *)
+  0xa94313e3;       (* arm_LDP X3 X4 SP (Immediate_Offset (iword (&48))) *)
+  0xa94243ef;       (* arm_LDP X15 X16 SP (Immediate_Offset (iword (&32))) *)
+  0xeb0f0063;       (* arm_SUBS X3 X3 X15 *)
+  0xfa100084;       (* arm_SBCS X4 X4 X16 *)
+  0xda9f23f0;       (* arm_CSETM X16 Condition_CC *)
+  0xa94603ef;       (* arm_LDP X15 X0 SP (Immediate_Offset (iword (&96))) *)
+  0xeb0501e5;       (* arm_SUBS X5 X15 X5 *)
+  0xfa060006;       (* arm_SBCS X6 X0 X6 *)
+  0xda9f23e0;       (* arm_CSETM X0 Condition_CC *)
+  0xca100063;       (* arm_EOR X3 X3 X16 *)
+  0xeb100063;       (* arm_SUBS X3 X3 X16 *)
+  0xca100084;       (* arm_EOR X4 X4 X16 *)
+  0xda100084;       (* arm_SBC X4 X4 X16 *)
+  0xca0000a5;       (* arm_EOR X5 X5 X0 *)
+  0xeb0000a5;       (* arm_SUBS X5 X5 X0 *)
+  0xca0000c6;       (* arm_EOR X6 X6 X0 *)
+  0xda0000c6;       (* arm_SBC X6 X6 X0 *)
+  0xca100010;       (* arm_EOR X16 X0 X16 *)
+  0xab09016b;       (* arm_ADDS X11 X11 X9 *)
+  0xba0a018c;       (* arm_ADCS X12 X12 X10 *)
+  0xba1f01ad;       (* arm_ADCS X13 X13 XZR *)
+  0x9a1f01ce;       (* arm_ADC X14 X14 XZR *)
+  0x9b057c62;       (* arm_MUL X2 X3 X5 *)
+  0x9bc57c60;       (* arm_UMULH X0 X3 X5 *)
+  0x9b067c8f;       (* arm_MUL X15 X4 X6 *)
+  0x9bc67c81;       (* arm_UMULH X1 X4 X6 *)
+  0xeb030084;       (* arm_SUBS X4 X4 X3 *)
+  0xda842484;       (* arm_CNEG X4 X4 Condition_CC *)
+  0xda9f23e9;       (* arm_CSETM X9 Condition_CC *)
+  0xab0001ef;       (* arm_ADDS X15 X15 X0 *)
+  0x9a1f0021;       (* arm_ADC X1 X1 XZR *)
+  0xeb0600a6;       (* arm_SUBS X6 X5 X6 *)
+  0xda8624c6;       (* arm_CNEG X6 X6 Condition_CC *)
+  0xda892129;       (* arm_CINV X9 X9 Condition_CC *)
+  0x9b067c85;       (* arm_MUL X5 X4 X6 *)
+  0x9bc67c86;       (* arm_UMULH X6 X4 X6 *)
+  0xab0f0040;       (* arm_ADDS X0 X2 X15 *)
+  0xba0101ef;       (* arm_ADCS X15 X15 X1 *)
+  0x9a1f0021;       (* arm_ADC X1 X1 XZR *)
+  0xb100053f;       (* arm_CMN X9 (rvalue (word 1)) *)
+  0xca0900a5;       (* arm_EOR X5 X5 X9 *)
+  0xba0000a0;       (* arm_ADCS X0 X5 X0 *)
+  0xca0900c6;       (* arm_EOR X6 X6 X9 *)
+  0xba0f00cf;       (* arm_ADCS X15 X6 X15 *)
+  0x9a090021;       (* arm_ADC X1 X1 X9 *)
+  0xab070169;       (* arm_ADDS X9 X11 X7 *)
+  0xba08018a;       (* arm_ADCS X10 X12 X8 *)
+  0xba0b01ab;       (* arm_ADCS X11 X13 X11 *)
+  0xba0c01cc;       (* arm_ADCS X12 X14 X12 *)
+  0xba1f01ad;       (* arm_ADCS X13 X13 XZR *)
+  0x9a1f01ce;       (* arm_ADC X14 X14 XZR *)
+  0xb100061f;       (* arm_CMN X16 (rvalue (word 1)) *)
+  0xca100042;       (* arm_EOR X2 X2 X16 *)
+  0xba090049;       (* arm_ADCS X9 X2 X9 *)
+  0xca100000;       (* arm_EOR X0 X0 X16 *)
+  0xba0a000a;       (* arm_ADCS X10 X0 X10 *)
+  0xca1001ef;       (* arm_EOR X15 X15 X16 *)
+  0xba0b01eb;       (* arm_ADCS X11 X15 X11 *)
+  0xca100021;       (* arm_EOR X1 X1 X16 *)
+  0xba0c002c;       (* arm_ADCS X12 X1 X12 *)
+  0xba1001ad;       (* arm_ADCS X13 X13 X16 *)
+  0x9a1001ce;       (* arm_ADC X14 X14 X16 *)
+  0xd28004c3;       (* arm_MOV X3 (rvalue (word 38)) *)
+  0x92407d65;       (* arm_AND X5 X11 (rvalue (word 4294967295)) *)
+  0xd360fd64;       (* arm_LSR X4 X11 32 *)
+  0x9b057c65;       (* arm_MUL X5 X3 X5 *)
+  0x9b047c64;       (* arm_MUL X4 X3 X4 *)
+  0xab0500e7;       (* arm_ADDS X7 X7 X5 *)
+  0x92407d85;       (* arm_AND X5 X12 (rvalue (word 4294967295)) *)
+  0xd360fd8c;       (* arm_LSR X12 X12 32 *)
+  0x9b057c65;       (* arm_MUL X5 X3 X5 *)
+  0x9b0c7c6c;       (* arm_MUL X12 X3 X12 *)
+  0xba050108;       (* arm_ADCS X8 X8 X5 *)
+  0x92407da5;       (* arm_AND X5 X13 (rvalue (word 4294967295)) *)
+  0xd360fdad;       (* arm_LSR X13 X13 32 *)
+  0x9b057c65;       (* arm_MUL X5 X3 X5 *)
+  0x9b0d7c6d;       (* arm_MUL X13 X3 X13 *)
+  0xba050129;       (* arm_ADCS X9 X9 X5 *)
+  0x92407dc5;       (* arm_AND X5 X14 (rvalue (word 4294967295)) *)
+  0xd360fdce;       (* arm_LSR X14 X14 32 *)
+  0x9b057c65;       (* arm_MUL X5 X3 X5 *)
+  0x9b0e7c6e;       (* arm_MUL X14 X3 X14 *)
+  0xba05014a;       (* arm_ADCS X10 X10 X5 *)
+  0x9a9f37eb;       (* arm_CSET X11 Condition_CS *)
+  0xd3607c85;       (* arm_LSL X5 X4 32 *)
+  0xab0500e7;       (* arm_ADDS X7 X7 X5 *)
+  0x93c48185;       (* arm_EXTR X5 X12 X4 32 *)
+  0xba050108;       (* arm_ADCS X8 X8 X5 *)
+  0x93cc81a5;       (* arm_EXTR X5 X13 X12 32 *)
+  0xba050129;       (* arm_ADCS X9 X9 X5 *)
+  0x93cd81c5;       (* arm_EXTR X5 X14 X13 32 *)
+  0xba05014a;       (* arm_ADCS X10 X10 X5 *)
+  0xd360fdc5;       (* arm_LSR X5 X14 32 *)
+  0x9a05016b;       (* arm_ADC X11 X11 X5 *)
+  0xab0a015f;       (* arm_CMN X10 X10 *)
+  0xb241014a;       (* arm_ORR X10 X10 (rvalue (word 9223372036854775808)) *)
+  0x9a0b0160;       (* arm_ADC X0 X11 X11 *)
+  0xd2800263;       (* arm_MOV X3 (rvalue (word 19)) *)
+  0x9b000c65;       (* arm_MADD X5 X3 X0 X3 *)
+  0xab0500e7;       (* arm_ADDS X7 X7 X5 *)
+  0xba1f0108;       (* arm_ADCS X8 X8 XZR *)
+  0xba1f0129;       (* arm_ADCS X9 X9 XZR *)
+  0xba1f014a;       (* arm_ADCS X10 X10 XZR *)
+  0x9a9f3063;       (* arm_CSEL X3 X3 XZR Condition_CC *)
+  0xeb0300e7;       (* arm_SUBS X7 X7 X3 *)
+  0xfa1f0108;       (* arm_SBCS X8 X8 XZR *)
+  0xfa1f0129;       (* arm_SBCS X9 X9 XZR *)
+  0xda1f014a;       (* arm_SBC X10 X10 XZR *)
+  0x9240f94a;       (* arm_AND X10 X10 (rvalue (word 9223372036854775807)) *)
+  0xa9042227;       (* arm_STP X7 X8 X17 (Immediate_Offset (iword (&64))) *)
+  0xa9052a29;       (* arm_STP X9 X10 X17 (Immediate_Offset (iword (&80))) *)
   0x910303ff;       (* arm_ADD SP SP (rvalue (word 192)) *)
   0xa8c153f3;       (* arm_LDP X19 X20 SP (Postimmediate_Offset (iword (&16))) *)
   0xd65f03c0        (* arm_RET X30 *)
 ];;
 
-let EDWARDS25519_PEPADD_EXEC = ARM_MK_EXEC_RULE edwards25519_pepadd_mc;;
+let EDWARDS25519_EPADD_EXEC = ARM_MK_EXEC_RULE edwards25519_epadd_mc;;
 
 (* ------------------------------------------------------------------------- *)
 (* Abbreviations used to state the specification.                            *)
@@ -1253,13 +1607,6 @@ let p_25519 = define `p_25519 = 578960446186580977117854925043439539266349923328
 let edwards25519_exprojective = define
  `edwards25519_exprojective P (X,Y,Z,W) <=>
         exprojective (integer_mod_ring p_25519) P (&X,&Y,&Z,&W)`;;
-
-let edwards25519_epprojective = define
- `edwards25519_epprojective (x,y) (YMX,XPY,KXY) <=>
-        x < &p_25519 /\ y < &p_25519 /\
-        &YMX = (y - x) rem &p_25519 /\
-        &XPY = (x + y) rem &p_25519 /\
-        &KXY = (&2 * &d_25519 * x * y) rem &p_25519`;;
 
 let EDWARDS25519_EXPROJECTIVE_BOUND = prove
  (`!x y X Y Z W.
@@ -1380,9 +1727,10 @@ let lvs =
   "y_1",[`X19`;`32`];
   "z_1",[`X19`;`64`];
   "w_1",[`X19`;`96`];
-  "ymx_2",[`X20`;`0`];
-  "xpy_2",[`X20`;`32`];
-  "kxy_2",[`X20`;`64`];
+  "x_2",[`X20`;`0`];
+  "y_2",[`X20`;`32`];
+  "z_2",[`X20`;`64`];
+  "w_2",[`X20`;`96`];
   "x_3",[`X17`;`0`];
   "y_3",[`X17`;`32`];
   "z_3",[`X17`;`64`];
@@ -1399,16 +1747,16 @@ let lvs =
 (* ------------------------------------------------------------------------- *)
 
 let LOCAL_MUL_P25519_TAC =
-  ARM_MACRO_SIM_ABBREV_TAC edwards25519_pepadd_mc 161 lvs
+  ARM_MACRO_SIM_ABBREV_TAC edwards25519_epadd_mc 161 lvs
    `!(t:armstate) pcin pcout p3 n3 p1 n1 p2 n2.
       !m. read(memory :> bytes(word_add (read p1 t) (word n1),8 * 4)) t = m
       ==>
       !n. read(memory :> bytes(word_add (read p2 t) (word n2),8 * 4)) t = n
       ==>
       aligned 16 (read SP t) /\
-      nonoverlapping (word pc,0x12fc) (word_add (read p3 t) (word n3),8 * 4)
+      nonoverlapping (word pc,0x1884) (word_add (read p3 t) (word n3),8 * 4)
       ==> ensures arm
-           (\s. aligned_bytes_loaded s (word pc) edwards25519_pepadd_mc /\
+           (\s. aligned_bytes_loaded s (word pc) edwards25519_epadd_mc /\
                 read PC s = pcin /\
                 read SP s = read SP t /\
                 read X17 s = read X17 t /\
@@ -1431,7 +1779,7 @@ let LOCAL_MUL_P25519_TAC =
 
   (*** First nested block multiplying the lower halves ***)
 
-  ARM_ACCSTEPS_TAC EDWARDS25519_PEPADD_EXEC
+  ARM_ACCSTEPS_TAC EDWARDS25519_EPADD_EXEC
    [3;5;10;11;15;17;18;19;22;24;25] (1--25) THEN
   RULE_ASSUM_TAC(REWRITE_RULE[lemma0; lemma1]) THEN
 
@@ -1450,7 +1798,7 @@ let LOCAL_MUL_P25519_TAC =
 
   (*** Second nested block multiplying the upper halves ***)
 
-  ARM_ACCSTEPS_TAC EDWARDS25519_PEPADD_EXEC
+  ARM_ACCSTEPS_TAC EDWARDS25519_EPADD_EXEC
    [28;30;35;36;40;42;43;44;47;49;50] (26--50) THEN
   RULE_ASSUM_TAC(REWRITE_RULE[lemma0; lemma1]) THEN
 
@@ -1467,7 +1815,7 @@ let LOCAL_MUL_P25519_TAC =
 
   (*** The sign-magnitude difference computation ***)
 
-  ARM_ACCSTEPS_TAC EDWARDS25519_PEPADD_EXEC
+  ARM_ACCSTEPS_TAC EDWARDS25519_EPADD_EXEC
     [53;54; 57;58; 61;63; 65;67] (51--68) THEN
   RULE_ASSUM_TAC(REWRITE_RULE[WORD_UNMASK_64]) THEN
 
@@ -1535,7 +1883,7 @@ let LOCAL_MUL_P25519_TAC =
 
   (*** The augmented H' = H + L_top ***)
 
-  ARM_ACCSTEPS_TAC EDWARDS25519_PEPADD_EXEC (69--72) (69--72) THEN
+  ARM_ACCSTEPS_TAC EDWARDS25519_EPADD_EXEC (69--72) (69--72) THEN
   MAP_EVERY ABBREV_TAC
    [`q2 = bignum_of_wordlist[sum_s69;sum_s70]`;
     `q3 = bignum_of_wordlist[sum_s71;sum_s72]`] THEN
@@ -1558,7 +1906,7 @@ let LOCAL_MUL_P25519_TAC =
 
   (*** Third nested block multiplying the absolute differences ***)
 
-  ARM_ACCSTEPS_TAC EDWARDS25519_PEPADD_EXEC
+  ARM_ACCSTEPS_TAC EDWARDS25519_EPADD_EXEC
    [73;75;80;81;85;87;88;89;92;94;95] (73--95) THEN
   RULE_ASSUM_TAC(REWRITE_RULE[lemma0; lemma1]) THEN
   SUBGOAL_THEN
@@ -1573,7 +1921,7 @@ let LOCAL_MUL_P25519_TAC =
 
   (*** The rest of the basic 4x4->8 multiply computation and its proof ***)
 
-  ARM_ACCSTEPS_TAC EDWARDS25519_PEPADD_EXEC
+  ARM_ACCSTEPS_TAC EDWARDS25519_EPADD_EXEC
    [96;97;98;99;100;101;104;106;108;110;111;112] (96--112) THEN
   MAP_EVERY ABBREV_TAC
    [`l = bignum_of_wordlist[mullo_s3; sum_s22; sum_s104; sum_s106]`;
@@ -1637,7 +1985,7 @@ let LOCAL_MUL_P25519_TAC =
 
   (*** Reduction from 8 digits to 5 digits ***)
 
-  ARM_ACCSTEPS_TAC EDWARDS25519_PEPADD_EXEC
+  ARM_ACCSTEPS_TAC EDWARDS25519_EPADD_EXEC
    [116;117;118;121;122;123;126;127;128;131;132;133;136;138;140;142;144]
    (113--144) THEN
 
@@ -1681,7 +2029,7 @@ let LOCAL_MUL_P25519_TAC =
 
   (*** Quotient estimate computation ***)
 
-  ARM_ACCSTEPS_TAC EDWARDS25519_PEPADD_EXEC (145--147) (145--147) THEN
+  ARM_ACCSTEPS_TAC EDWARDS25519_EPADD_EXEC (145--147) (145--147) THEN
   ABBREV_TAC `t = bignum_of_wordlist
    [sum_s136; sum_s138; sum_s140;
     word_or sum_s142 (word 9223372036854775808)]` THEN
@@ -1729,7 +2077,7 @@ let LOCAL_MUL_P25519_TAC =
     ACCUMULATOR_POP_ASSUM_LIST(MP_TAC o end_itlist CONJ o DESUM_RULE) THEN
     DISCH_THEN(fun th -> REWRITE_TAC[th]) THEN REAL_INTEGER_TAC;
     ACCUMULATOR_POP_ASSUM_LIST(K ALL_TAC)] THEN
-  ARM_STEPS_TAC EDWARDS25519_PEPADD_EXEC (159--160) THEN
+  ARM_STEPS_TAC EDWARDS25519_EPADD_EXEC (159--160) THEN
   ABBREV_TAC `qm:int64 = word(19 + 19 * val(sum_s147:int64))` THEN
   SUBGOAL_THEN `&(val(qm:int64)):real = &19 * (&(val(sum_s147:int64)) + &1)`
   ASSUME_TAC THENL
@@ -1742,7 +2090,7 @@ let LOCAL_MUL_P25519_TAC =
 
   (*** The rest of the computation ***)
 
-  ARM_ACCSTEPS_TAC EDWARDS25519_PEPADD_EXEC (150--161) (150--161) THEN
+  ARM_ACCSTEPS_TAC EDWARDS25519_EPADD_EXEC (150--161) (150--161) THEN
   ENSURES_FINAL_STATE_TAC THEN ASM_REWRITE_TAC[] THEN
   CONV_TAC(LAND_CONV BIGNUM_EXPAND_CONV) THEN ASM_REWRITE_TAC[] THEN
   CONV_TAC SYM_CONV THEN MATCH_MP_TAC MOD_UNIQ_BALANCED_REAL THEN
@@ -1780,16 +2128,16 @@ let LOCAL_MUL_P25519_TAC =
 (* ------------------------------------------------------------------------- *)
 
 let LOCAL_MUL_4_TAC =
-  ARM_MACRO_SIM_ABBREV_TAC edwards25519_pepadd_mc 155 lvs
+  ARM_MACRO_SIM_ABBREV_TAC edwards25519_epadd_mc 155 lvs
    `!(t:armstate) pcin pcout p3 n3 p1 n1 p2 n2.
       !m. read(memory :> bytes(word_add (read p1 t) (word n1),8 * 4)) t = m
       ==>
       !n. read(memory :> bytes(word_add (read p2 t) (word n2),8 * 4)) t = n
       ==>
       aligned 16 (read SP t) /\
-      nonoverlapping (word pc,0x12fc) (word_add (read p3 t) (word n3),8 * 4)
+      nonoverlapping (word pc,0x1884) (word_add (read p3 t) (word n3),8 * 4)
       ==> ensures arm
-           (\s. aligned_bytes_loaded s (word pc) edwards25519_pepadd_mc /\
+           (\s. aligned_bytes_loaded s (word pc) edwards25519_epadd_mc /\
                 read PC s = pcin /\
                 read SP s = read SP t /\
                 read X17 s = read X17 t /\
@@ -1814,7 +2162,7 @@ let LOCAL_MUL_4_TAC =
 
   (*** First nested block multiplying the lower halves ***)
 
-  ARM_ACCSTEPS_TAC EDWARDS25519_PEPADD_EXEC
+  ARM_ACCSTEPS_TAC EDWARDS25519_EPADD_EXEC
    [3;5;10;11;15;17;18;19;22;24;25] (1--25) THEN
   RULE_ASSUM_TAC(REWRITE_RULE[lemma0; lemma1]) THEN
 
@@ -1833,7 +2181,7 @@ let LOCAL_MUL_4_TAC =
 
   (*** Second nested block multiplying the upper halves ***)
 
-  ARM_ACCSTEPS_TAC EDWARDS25519_PEPADD_EXEC
+  ARM_ACCSTEPS_TAC EDWARDS25519_EPADD_EXEC
    [28;30;35;36;40;42;43;44;47;49;50] (26--50) THEN
   RULE_ASSUM_TAC(REWRITE_RULE[lemma0; lemma1]) THEN
 
@@ -1850,7 +2198,7 @@ let LOCAL_MUL_4_TAC =
 
   (*** The sign-magnitude difference computation ***)
 
-  ARM_ACCSTEPS_TAC EDWARDS25519_PEPADD_EXEC
+  ARM_ACCSTEPS_TAC EDWARDS25519_EPADD_EXEC
     [53;54; 57;58; 61;63; 65;67] (51--68) THEN
   RULE_ASSUM_TAC(REWRITE_RULE[WORD_UNMASK_64]) THEN
 
@@ -1918,7 +2266,7 @@ let LOCAL_MUL_4_TAC =
 
   (*** The augmented H' = H + L_top ***)
 
-  ARM_ACCSTEPS_TAC EDWARDS25519_PEPADD_EXEC (69--72) (69--72) THEN
+  ARM_ACCSTEPS_TAC EDWARDS25519_EPADD_EXEC (69--72) (69--72) THEN
   MAP_EVERY ABBREV_TAC
    [`q2 = bignum_of_wordlist[sum_s69;sum_s70]`;
     `q3 = bignum_of_wordlist[sum_s71;sum_s72]`] THEN
@@ -1941,7 +2289,7 @@ let LOCAL_MUL_4_TAC =
 
   (*** Third nested block multiplying the absolute differences ***)
 
-  ARM_ACCSTEPS_TAC EDWARDS25519_PEPADD_EXEC
+  ARM_ACCSTEPS_TAC EDWARDS25519_EPADD_EXEC
    [73;75;80;81;85;87;88;89;92;94;95] (73--95) THEN
   RULE_ASSUM_TAC(REWRITE_RULE[lemma0; lemma1]) THEN
   SUBGOAL_THEN
@@ -1956,7 +2304,7 @@ let LOCAL_MUL_4_TAC =
 
   (*** The rest of the basic 4x4->8 multiply computation and its proof ***)
 
-  ARM_ACCSTEPS_TAC EDWARDS25519_PEPADD_EXEC
+  ARM_ACCSTEPS_TAC EDWARDS25519_EPADD_EXEC
    [96;97;98;99;100;101;104;106;108;110;111;112] (96--112) THEN
   MAP_EVERY ABBREV_TAC
    [`l = bignum_of_wordlist[mullo_s3; sum_s22; sum_s104; sum_s106]`;
@@ -2021,7 +2369,7 @@ let LOCAL_MUL_4_TAC =
 
   (*** Reduction from 8 digits to 5 digits ***)
 
-  ARM_ACCSTEPS_TAC EDWARDS25519_PEPADD_EXEC
+  ARM_ACCSTEPS_TAC EDWARDS25519_EPADD_EXEC
    [116;117;118;121;122;123;126;127;128;131;132;133;136;138;140;142;144]
    (113--144) THEN
 
@@ -2065,7 +2413,7 @@ let LOCAL_MUL_4_TAC =
 
   (*** Quotient estimate computation ***)
 
-  ARM_ACCSTEPS_TAC EDWARDS25519_PEPADD_EXEC (145--147) (145--147) THEN
+  ARM_ACCSTEPS_TAC EDWARDS25519_EPADD_EXEC (145--147) (145--147) THEN
   SUBGOAL_THEN `ca DIV 2 EXP 255 = val(sum_s147:int64)`
    (fun th -> SUBST_ALL_TAC th THEN ASSUME_TAC th)
   THENL
@@ -2085,7 +2433,7 @@ let LOCAL_MUL_4_TAC =
     ACCUMULATOR_POP_ASSUM_LIST(MP_TAC o end_itlist CONJ o DESUM_RULE) THEN
     DISCH_THEN(fun th -> REWRITE_TAC[th]) THEN REAL_INTEGER_TAC;
     ACCUMULATOR_POP_ASSUM_LIST(K ALL_TAC)] THEN
-  ARM_STEPS_TAC EDWARDS25519_PEPADD_EXEC (89--90) THEN
+  ARM_STEPS_TAC EDWARDS25519_EPADD_EXEC (89--90) THEN
   ABBREV_TAC `qm:int64 = word(0 + 19 * val(sum_s147:int64))` THEN
   SUBGOAL_THEN `&(val(qm:int64)):real = &19 * &(val(sum_s147:int64))`
   ASSUME_TAC THENL
@@ -2098,7 +2446,7 @@ let LOCAL_MUL_4_TAC =
 
   (*** The rest of the computation ***)
 
-  ARM_ACCSTEPS_TAC EDWARDS25519_PEPADD_EXEC (150--153) (150--155) THEN
+  ARM_ACCSTEPS_TAC EDWARDS25519_EPADD_EXEC (150--153) (150--155) THEN
   ENSURES_FINAL_STATE_TAC THEN ASM_REWRITE_TAC[] THEN
   REWRITE_TAC[GSYM CONG; num_congruent] THEN
   REWRITE_TAC[GSYM INT_OF_NUM_CLAUSES] THEN
@@ -2148,16 +2496,16 @@ let LOCAL_MUL_4_TAC =
 (* ------------------------------------------------------------------------- *)
 
 let LOCAL_ADD_4_TAC =
-  ARM_MACRO_SIM_ABBREV_TAC edwards25519_pepadd_mc 10 lvs
+  ARM_MACRO_SIM_ABBREV_TAC edwards25519_epadd_mc 10 lvs
    `!(t:armstate) pcin pcout p3 n3 p1 n1 p2 n2.
       !m. read(memory :> bytes(word_add (read p1 t) (word n1),8 * 4)) t = m
       ==>
       !n. read(memory :> bytes(word_add (read p2 t) (word n2),8 * 4)) t = n
       ==>
       aligned 16 (read SP t) /\
-      nonoverlapping (word pc,0x12fc) (word_add (read p3 t) (word n3),8 * 4)
+      nonoverlapping (word pc,0x1884) (word_add (read p3 t) (word n3),8 * 4)
       ==> ensures arm
-           (\s. aligned_bytes_loaded s (word pc) edwards25519_pepadd_mc /\
+           (\s. aligned_bytes_loaded s (word pc) edwards25519_epadd_mc /\
                 read PC s = pcin /\
                 read SP s = read SP t /\
                 read X17 s = read X17 t /\
@@ -2177,7 +2525,7 @@ let LOCAL_ADD_4_TAC =
   REWRITE_TAC[BIGNUM_FROM_MEMORY_BYTES] THEN ENSURES_INIT_TAC "s0" THEN
   FIRST_ASSUM(BIGNUM_LDIGITIZE_TAC "n_" o lhand o concl) THEN
   FIRST_ASSUM(BIGNUM_LDIGITIZE_TAC "m_" o lhand o concl) THEN
-  ARM_ACCSTEPS_TAC EDWARDS25519_PEPADD_EXEC [3;4;7;8] (1--10) THEN
+  ARM_ACCSTEPS_TAC EDWARDS25519_EPADD_EXEC [3;4;7;8] (1--10) THEN
   ENSURES_FINAL_STATE_TAC THEN ASM_REWRITE_TAC[] THEN DISCH_TAC THEN
   CONV_TAC(LAND_CONV BIGNUM_LEXPAND_CONV) THEN ASM_REWRITE_TAC[] THEN
   MATCH_MP_TAC CONG_IMP_EQ THEN EXISTS_TAC `2 EXP 256` THEN
@@ -2196,14 +2544,14 @@ let LOCAL_ADD_4_TAC =
 (* ------------------------------------------------------------------------- *)
 
 let LOCAL_DOUBLE_4_TAC =
-  ARM_MACRO_SIM_ABBREV_TAC edwards25519_pepadd_mc 8 lvs
+  ARM_MACRO_SIM_ABBREV_TAC edwards25519_epadd_mc 8 lvs
    `!(t:armstate) pcin pcout p3 n3 p1 n1.
       !n. read(memory :> bytes(word_add (read p1 t) (word n1),8 * 4)) t = n
       ==>
       aligned 16 (read SP t) /\
-      nonoverlapping (word pc,0x12fc) (word_add (read p3 t) (word n3),8 * 4)
+      nonoverlapping (word pc,0x1884) (word_add (read p3 t) (word n3),8 * 4)
       ==> ensures arm
-           (\s. aligned_bytes_loaded s (word pc) edwards25519_pepadd_mc /\
+           (\s. aligned_bytes_loaded s (word pc) edwards25519_epadd_mc /\
                 read PC s = pcin /\
                 read SP s = read SP t /\
                 read X17 s = read X17 t /\
@@ -2221,7 +2569,7 @@ let LOCAL_DOUBLE_4_TAC =
   DISCH_THEN(REPEAT_TCL CONJUNCTS_THEN ASSUME_TAC) THEN
   REWRITE_TAC[BIGNUM_FROM_MEMORY_BYTES] THEN ENSURES_INIT_TAC "s0" THEN
   FIRST_ASSUM(BIGNUM_LDIGITIZE_TAC "n_" o lhand o concl) THEN
-  ARM_ACCSTEPS_TAC EDWARDS25519_PEPADD_EXEC [2;3;5;6] (1--8) THEN
+  ARM_ACCSTEPS_TAC EDWARDS25519_EPADD_EXEC [2;3;5;6] (1--8) THEN
   ENSURES_FINAL_STATE_TAC THEN ASM_REWRITE_TAC[] THEN DISCH_TAC THEN
   CONV_TAC(LAND_CONV BIGNUM_LEXPAND_CONV) THEN ASM_REWRITE_TAC[] THEN
   MATCH_MP_TAC CONG_IMP_EQ THEN EXISTS_TAC `2 EXP 256` THEN
@@ -2239,16 +2587,16 @@ let LOCAL_DOUBLE_4_TAC =
 (* ------------------------------------------------------------------------- *)
 
 let LOCAL_SUB_4_TAC =
-  ARM_MACRO_SIM_ABBREV_TAC edwards25519_pepadd_mc 16 lvs
+  ARM_MACRO_SIM_ABBREV_TAC edwards25519_epadd_mc 16 lvs
    `!(t:armstate) pcin pcout p3 n3 p1 n1 p2 n2.
       !m. read(memory :> bytes(word_add (read p1 t) (word n1),8 * 4)) t = m
       ==>
       !n. read(memory :> bytes(word_add (read p2 t) (word n2),8 * 4)) t = n
       ==>
       aligned 16 (read SP t) /\
-      nonoverlapping (word pc,0x12fc) (word_add (read p3 t) (word n3),8 * 4)
+      nonoverlapping (word pc,0x1884) (word_add (read p3 t) (word n3),8 * 4)
       ==> ensures arm
-           (\s. aligned_bytes_loaded s (word pc) edwards25519_pepadd_mc /\
+           (\s. aligned_bytes_loaded s (word pc) edwards25519_epadd_mc /\
                 read PC s = pcin /\
                 read SP s = read SP t /\
                 read X17 s = read X17 t /\
@@ -2271,7 +2619,7 @@ let LOCAL_SUB_4_TAC =
   REWRITE_TAC[BIGNUM_FROM_MEMORY_BYTES] THEN ENSURES_INIT_TAC "s0" THEN
   FIRST_ASSUM(BIGNUM_LDIGITIZE_TAC "n_" o lhand o concl) THEN
   FIRST_ASSUM(BIGNUM_LDIGITIZE_TAC "m_" o lhand o concl) THEN
-  ARM_ACCSTEPS_TAC EDWARDS25519_PEPADD_EXEC
+  ARM_ACCSTEPS_TAC EDWARDS25519_EPADD_EXEC
    [3;4;7;8;10;11;12;14] (1--16) THEN
   ENSURES_FINAL_STATE_TAC THEN ASM_REWRITE_TAC[] THEN DISCH_TAC THEN
   MATCH_MP_TAC(MESON[INT_OF_NUM_LT]
@@ -2307,16 +2655,16 @@ let LOCAL_SUB_4_TAC =
 (* ------------------------------------------------------------------------- *)
 
 let LOCAL_ADD_TWICE4_TAC =
-  ARM_MACRO_SIM_ABBREV_TAC edwards25519_pepadd_mc 16 lvs
+  ARM_MACRO_SIM_ABBREV_TAC edwards25519_epadd_mc 16 lvs
    `!(t:armstate) pcin pcout p3 n3 p1 n1 p2 n2.
       !m. read(memory :> bytes(word_add (read p1 t) (word n1),8 * 4)) t = m
       ==>
       !n. read(memory :> bytes(word_add (read p2 t) (word n2),8 * 4)) t = n
       ==>
       aligned 16 (read SP t) /\
-      nonoverlapping (word pc,0x12fc) (word_add (read p3 t) (word n3),8 * 4)
+      nonoverlapping (word pc,0x1884) (word_add (read p3 t) (word n3),8 * 4)
       ==> ensures arm
-           (\s. aligned_bytes_loaded s (word pc) edwards25519_pepadd_mc /\
+           (\s. aligned_bytes_loaded s (word pc) edwards25519_epadd_mc /\
                 read PC s = pcin /\
                 read SP s = read SP t /\
                 read X17 s = read X17 t /\
@@ -2336,7 +2684,7 @@ let LOCAL_ADD_TWICE4_TAC =
   REWRITE_TAC[BIGNUM_FROM_MEMORY_BYTES] THEN ENSURES_INIT_TAC "s0" THEN
   FIRST_ASSUM(BIGNUM_LDIGITIZE_TAC "n_" o lhand o concl) THEN
   FIRST_ASSUM(BIGNUM_LDIGITIZE_TAC "m_" o lhand o concl) THEN
-  ARM_ACCSTEPS_TAC EDWARDS25519_PEPADD_EXEC (1--8) (1--8) THEN
+  ARM_ACCSTEPS_TAC EDWARDS25519_EPADD_EXEC (1--8) (1--8) THEN
   SUBGOAL_THEN `carry_s8 <=> 2 EXP 256 <= m + n` SUBST_ALL_TAC THENL
    [MATCH_MP_TAC FLAG_FROM_CARRY_LE THEN EXISTS_TAC `256` THEN
     MAP_EVERY EXPAND_TAC ["m"; "n"] THEN REWRITE_TAC[GSYM REAL_OF_NUM_ADD] THEN
@@ -2344,7 +2692,7 @@ let LOCAL_ADD_TWICE4_TAC =
     ACCUMULATOR_ASSUM_LIST(MP_TAC o end_itlist CONJ o DECARRY_RULE) THEN
     DISCH_THEN(fun th -> REWRITE_TAC[th]) THEN BOUNDER_TAC[];
     ALL_TAC] THEN
-  ARM_ACCSTEPS_TAC EDWARDS25519_PEPADD_EXEC (11--14) (9--16) THEN
+  ARM_ACCSTEPS_TAC EDWARDS25519_EPADD_EXEC (11--14) (9--16) THEN
   ENSURES_FINAL_STATE_TAC THEN ASM_REWRITE_TAC[] THEN DISCH_TAC THEN
   REWRITE_TAC[num_congruent; GSYM INT_OF_NUM_ADD] THEN
   MATCH_MP_TAC(MESON[INT_OF_NUM_LT]
@@ -2377,16 +2725,16 @@ let LOCAL_ADD_TWICE4_TAC =
 (* ------------------------------------------------------------------------- *)
 
 let LOCAL_SUB_TWICE4_TAC =
-  ARM_MACRO_SIM_ABBREV_TAC edwards25519_pepadd_mc 16 lvs
+  ARM_MACRO_SIM_ABBREV_TAC edwards25519_epadd_mc 16 lvs
    `!(t:armstate) pcin pcout p3 n3 p1 n1 p2 n2.
       !m. read(memory :> bytes(word_add (read p1 t) (word n1),8 * 4)) t = m
       ==>
       !n. read(memory :> bytes(word_add (read p2 t) (word n2),8 * 4)) t = n
       ==>
       aligned 16 (read SP t) /\
-      nonoverlapping (word pc,0x12fc) (word_add (read p3 t) (word n3),8 * 4)
+      nonoverlapping (word pc,0x1884) (word_add (read p3 t) (word n3),8 * 4)
       ==> ensures arm
-           (\s. aligned_bytes_loaded s (word pc) edwards25519_pepadd_mc /\
+           (\s. aligned_bytes_loaded s (word pc) edwards25519_epadd_mc /\
                 read PC s = pcin /\
                 read SP s = read SP t /\
                 read X17 s = read X17 t /\
@@ -2409,7 +2757,7 @@ let LOCAL_SUB_TWICE4_TAC =
   REWRITE_TAC[BIGNUM_FROM_MEMORY_BYTES] THEN ENSURES_INIT_TAC "s0" THEN
   FIRST_ASSUM(BIGNUM_LDIGITIZE_TAC "n_" o lhand o concl) THEN
   FIRST_ASSUM(BIGNUM_LDIGITIZE_TAC "m_" o lhand o concl) THEN
-  ARM_ACCSTEPS_TAC EDWARDS25519_PEPADD_EXEC (1--8) (1--8) THEN
+  ARM_ACCSTEPS_TAC EDWARDS25519_EPADD_EXEC (1--8) (1--8) THEN
   SUBGOAL_THEN `carry_s8 <=> m < n` SUBST_ALL_TAC THENL
    [MATCH_MP_TAC FLAG_FROM_CARRY_LT THEN EXISTS_TAC `256` THEN
     MAP_EVERY EXPAND_TAC ["m"; "n"] THEN REWRITE_TAC[GSYM REAL_OF_NUM_ADD] THEN
@@ -2417,7 +2765,7 @@ let LOCAL_SUB_TWICE4_TAC =
     ACCUMULATOR_ASSUM_LIST(MP_TAC o end_itlist CONJ o DECARRY_RULE) THEN
     DISCH_THEN(fun th -> REWRITE_TAC[th]) THEN BOUNDER_TAC[];
     ALL_TAC] THEN
-  ARM_ACCSTEPS_TAC EDWARDS25519_PEPADD_EXEC (11--14) (9--16) THEN
+  ARM_ACCSTEPS_TAC EDWARDS25519_EPADD_EXEC (11--14) (9--16) THEN
   ENSURES_FINAL_STATE_TAC THEN ASM_REWRITE_TAC[] THEN DISCH_TAC THEN
   MATCH_MP_TAC(MESON[INT_OF_NUM_LT]
    `!x':int. (x' == a) (mod p) /\ x' < &e /\ &x = x'
@@ -2450,24 +2798,24 @@ let LOCAL_SUB_TWICE4_TAC =
 (* Overall point operation proof.                                            *)
 (* ------------------------------------------------------------------------- *)
 
-let EDWARDS25519_PEPADD_CORRECT = time prove
- (`!p3 p1 Q1 p2 T2 pc stackpointer.
+let EDWARDS25519_EPADD_CORRECT = time prove
+ (`!p3 p1 Q1 p2 Q2 pc stackpointer.
     aligned 16 stackpointer /\
     ALL (nonoverlapping (stackpointer,192))
-        [(word pc,0x12fc); (p3,128); (p1,128); (p2,96)] /\
-    nonoverlapping (p3,128) (word pc,0x12fc)
+        [(word pc,0x1884); (p3,128); (p1,128); (p2,128)] /\
+    nonoverlapping (p3,128) (word pc,0x1884)
     ==> ensures arm
-         (\s. aligned_bytes_loaded s (word pc) edwards25519_pepadd_mc /\
+         (\s. aligned_bytes_loaded s (word pc) edwards25519_epadd_mc /\
               read PC s = word(pc + 0x8) /\
               read SP s = stackpointer /\
               C_ARGUMENTS [p3; p1; p2] s /\
               bignum_quadruple_from_memory (p1,4) s = Q1 /\
-              bignum_triple_from_memory(p2,4) s = T2)
-         (\s. read PC s = word (pc + 0x12f0) /\
+              bignum_quadruple_from_memory(p2,4) s = Q2)
+         (\s. read PC s = word (pc + 0x1878) /\
               !P1 P2. P1 IN group_carrier edwards25519_group /\
                       P2 IN group_carrier edwards25519_group /\
                       edwards25519_exprojective P1 Q1 /\
-                      edwards25519_epprojective P2 T2
+                      edwards25519_exprojective P2 Q2
                       ==> edwards25519_exprojective
                            (edwards_add edwards25519 P1 P2)
                            (bignum_quadruple_from_memory(p3,4) s))
@@ -2479,36 +2827,49 @@ let EDWARDS25519_PEPADD_CORRECT = time prove
   REWRITE_TAC[FORALL_PAIR_THM] THEN
   MAP_EVERY X_GEN_TAC
    [`p3:int64`; `p1:int64`; `X_1:num`; `Y_1:num`; `Z_1:num`; `W_1:num`;
-    `p2:int64`; `YMX_2:num`; `XPY_2:num`; `KXY_2:num`;
+    `p2:int64`; `X_2:num`; `Y_2:num`; `Z_2:num`; `W_2:num`;
     `pc:num`; `stackpointer:int64`] THEN
   REWRITE_TAC[ALLPAIRS; ALL; NONOVERLAPPING_CLAUSES] THEN STRIP_TAC THEN
-  REWRITE_TAC[C_ARGUMENTS; SOME_FLAGS;
-              bignum_quadruple_from_memory; bignum_triple_from_memory;
+  REWRITE_TAC[C_ARGUMENTS; SOME_FLAGS; bignum_quadruple_from_memory;
               bignum_pair_from_memory; PAIR_EQ] THEN
   CONV_TAC(ONCE_DEPTH_CONV NUM_MULT_CONV) THEN
   REWRITE_TAC[BIGNUM_FROM_MEMORY_BYTES] THEN ENSURES_INIT_TAC "s0" THEN
 
-  LOCAL_DOUBLE_4_TAC 3 ["t0"; "z_1"] THEN
+  LOCAL_MUL_4_TAC 3 ["t0"; "w_1"; "w_2"] THEN
   LOCAL_SUB_4_TAC 0 ["t1"; "y_1"; "x_1"] THEN
-  LOCAL_ADD_4_TAC 0 ["t2"; "y_1"; "x_1"] THEN
-  LOCAL_MUL_4_TAC 0 ["t3"; "w_1"; "kxy_2"] THEN
-  LOCAL_MUL_4_TAC 0 ["t1"; "t1"; "ymx_2"] THEN
-  LOCAL_MUL_4_TAC 0 ["t2"; "t2"; "xpy_2"] THEN
-  LOCAL_SUB_TWICE4_TAC 0 ["t4"; "t0"; "t3"] THEN
-  LOCAL_ADD_TWICE4_TAC 0 ["t0"; "t0"; "t3"] THEN
-  LOCAL_SUB_TWICE4_TAC 0 ["t5"; "t2"; "t1"] THEN
-  LOCAL_ADD_TWICE4_TAC 0 ["t1"; "t2"; "t1"] THEN
-  LOCAL_MUL_P25519_TAC 0 ["z_3"; "t4"; "t0"] THEN
-  LOCAL_MUL_P25519_TAC 0 ["x_3"; "t5"; "t4"] THEN
-  LOCAL_MUL_P25519_TAC 0 ["y_3"; "t0"; "t1"] THEN
-  LOCAL_MUL_P25519_TAC 0 ["w_3"; "t5"; "t1"] THEN
+  LOCAL_SUB_4_TAC 0 ["t2"; "y_2"; "x_2"] THEN
+  LOCAL_ADD_4_TAC 0 ["t3"; "y_1"; "x_1"] THEN
+  LOCAL_ADD_4_TAC 0 ["t4"; "y_2"; "x_2"] THEN
+  LOCAL_DOUBLE_4_TAC 0 ["t5"; "z_2"] THEN
+  LOCAL_MUL_4_TAC 0 ["t1"; "t1"; "t2"] THEN
+  LOCAL_MUL_4_TAC 0 ["t3"; "t3"; "t4"] THEN
+
+  ARM_STEPS_TAC EDWARDS25519_EPADD_EXEC (12--29) THEN
+  SUBGOAL_THEN
+   `read (memory :> bytes (word_add stackpointer (word 64),8 * 4)) s29 =
+    16295367250680780974490674513165176452449235426866156013048779062215315747161`
+  ASSUME_TAC THENL
+   [CONV_TAC(LAND_CONV BIGNUM_EXPAND_CONV) THEN ASM_REWRITE_TAC[] THEN
+    CONV_TAC(DEPTH_CONV WORD_NUM_RED_CONV);
+    ALL_TAC] THEN
+
+  LOCAL_MUL_4_TAC 0 ["t2"; "t2"; "t0"] THEN
+  LOCAL_MUL_4_TAC 0 ["t4"; "z_1"; "t5"] THEN
+  LOCAL_SUB_TWICE4_TAC 0 ["t0"; "t3"; "t1"] THEN
+  LOCAL_ADD_TWICE4_TAC 0 ["t5"; "t3"; "t1"] THEN
+  LOCAL_SUB_TWICE4_TAC 0 ["t1"; "t4"; "t2"] THEN
+  LOCAL_ADD_TWICE4_TAC 0 ["t3"; "t4"; "t2"] THEN
+  LOCAL_MUL_P25519_TAC 0 ["w_3"; "t0"; "t5"] THEN
+  LOCAL_MUL_P25519_TAC 0 ["x_3"; "t0"; "t1"] THEN
+  LOCAL_MUL_P25519_TAC 0 ["y_3"; "t3"; "t5"] THEN
+  LOCAL_MUL_P25519_TAC 0 ["z_3"; "t1"; "t3"] THEN
 
   ENSURES_FINAL_STATE_TAC THEN ASM_REWRITE_TAC[] THEN
-
   MAP_EVERY X_GEN_TAC [`x1:int`; `y1:int`; `x2:int`; `y2:int`] THEN
-  STRIP_TAC THEN
-  FIRST_ASSUM(STRIP_ASSUME_TAC o MATCH_MP EDWARDS25519_EXPROJECTIVE_BOUND) THEN
-  DISCARD_STATE_TAC "s17" THEN
+  STRIP_TAC THEN EVERY_ASSUM(fun th ->
+    try STRIP_ASSUME_TAC(MATCH_MP EDWARDS25519_EXPROJECTIVE_BOUND th)
+    with _ -> ALL_TAC) THEN
+  DISCARD_STATE_TAC "s39" THEN
   DISCARD_MATCHING_ASSUMPTIONS
    [`aligned a b`; `nonoverlapping_modulo a b c`] THEN
 
@@ -2534,7 +2895,7 @@ let EDWARDS25519_PEPADD_CORRECT = time prove
     `x1:int`; `y1:int`;
     `&X_1:int`; `&Y_1:int`; `&Z_1:int`; `&W_1:int`;
     `x2:int`; `y2:int`;
-    `x2:int`; `y2:int`; `&1:int`; `(x2 * y2) rem &p_25519`]
+    `&X_2:int`; `&Y_2:int`; `&Z_2:int`; `&W_2:int`]
    EDWARDS_EXPROJADD4) THEN
   ANTS_TAC THENL
    [REWRITE_TAC[EDWARDS_NONSINGULAR_25519] THEN
@@ -2542,7 +2903,8 @@ let EDWARDS25519_PEPADD_CORRECT = time prove
     SIMP_TAC[EDWARDS25519_GROUP] THEN
     REWRITE_TAC[edwards_curve] THEN STRIP_TAC THEN STRIP_TAC THEN
     REWRITE_TAC[FIELD_INTEGER_MOD_RING; PRIME_P25519] THEN
-    FIRST_X_ASSUM(MP_TAC o GEN_REWRITE_RULE I [edwards25519_exprojective]) THEN
+    REPEAT(FIRST_X_ASSUM(MP_TAC o
+     GEN_REWRITE_RULE I [edwards25519_exprojective])) THEN
     DISCH_THEN(fun th -> REWRITE_TAC[th]) THEN
     ASM_REWRITE_TAC[exprojective] THEN
     REWRITE_TAC[INTEGER_MOD_RING_CHAR; IN_INTEGER_MOD_RING_CARRIER;
@@ -2564,38 +2926,39 @@ let EDWARDS25519_PEPADD_CORRECT = time prove
   MATCH_MP_TAC EQ_IMP THEN AP_TERM_TAC THEN
   ONCE_REWRITE_TAC[GSYM MOD_MULT_MOD2] THEN
   ASM_REWRITE_TAC[GSYM INT_OF_NUM_REM; GSYM INT_OF_NUM_CLAUSES] THEN
-
-  FIRST_X_ASSUM(MP_TAC o GEN_REWRITE_RULE I [edwards25519_epprojective]) THEN
+  FIRST_X_ASSUM(MP_TAC o GEN_REWRITE_RULE I [edwards25519_exprojective]) THEN
   DISCH_THEN(fun th -> REWRITE_TAC[th]) THEN
-
   REWRITE_TAC[edwards_exprojadd4; edwards_exprojadd; edwards25519;
               INTEGER_MOD_RING_CLAUSES] THEN
   CONV_TAC(TOP_DEPTH_CONV let_CONV) THEN
   SUBGOAL_THEN `&e_25519 = (-- &1) rem &p_25519` SUBST_ALL_TAC THENL
    [REWRITE_TAC[e_25519; p_25519] THEN CONV_TAC INT_REDUCE_CONV; ALL_TAC] THEN
+  REWRITE_TAC[GSYM p_25519; GSYM INT_OF_NUM_REM; GSYM INT_OF_NUM_CLAUSES; GSYM
+   (CONV_RULE NUM_REDUCE_CONV (REWRITE_RULE[p_25519]
+     (AP_TERM `\x. (2 * x) MOD p_25519` d_25519)))] THEN
   CONV_TAC INT_REM_DOWN_CONV THEN
   REWRITE_TAC[PAIR_EQ] THEN CONV_TAC INT_REM_DOWN_CONV THEN
   REPEAT CONJ_TAC THEN AP_THM_TAC THEN AP_TERM_TAC THEN INT_ARITH_TAC);;
 
-let EDWARDS25519_PEPADD_SUBROUTINE_CORRECT = time prove
- (`!p3 p1 Q1 p2 T2 pc stackpointer returnaddress.
+let EDWARDS25519_EPADD_SUBROUTINE_CORRECT = time prove
+ (`!p3 p1 Q1 p2 Q2 pc stackpointer returnaddress.
     aligned 16 stackpointer /\
     ALL (nonoverlapping (word_sub stackpointer (word 208),208))
-        [(word pc,0x12fc); (p3,128); (p1,128); (p2,96)] /\
-    nonoverlapping (p3,128) (word pc,0x12fc)
+        [(word pc,0x1884); (p3,128); (p1,128); (p2,128)] /\
+    nonoverlapping (p3,128) (word pc,0x1884)
     ==> ensures arm
-         (\s. aligned_bytes_loaded s (word pc) edwards25519_pepadd_mc /\
+         (\s. aligned_bytes_loaded s (word pc) edwards25519_epadd_mc /\
               read PC s = word pc /\
               read SP s = stackpointer /\
               read X30 s = returnaddress /\
               C_ARGUMENTS [p3; p1; p2] s /\
               bignum_quadruple_from_memory (p1,4) s = Q1 /\
-              bignum_triple_from_memory (p2,4) s = T2)
+              bignum_quadruple_from_memory (p2,4) s = Q2)
          (\s. read PC s = returnaddress /\
               !P1 P2. P1 IN group_carrier edwards25519_group /\
                       P2 IN group_carrier edwards25519_group /\
                       edwards25519_exprojective P1 Q1 /\
-                      edwards25519_epprojective P2 T2
+                      edwards25519_exprojective P2 Q2
                       ==> edwards25519_exprojective
                            (edwards_add edwards25519 P1 P2)
                            (bignum_quadruple_from_memory(p3,4) s))
@@ -2604,5 +2967,5 @@ let EDWARDS25519_PEPADD_SUBROUTINE_CORRECT = time prove
            MAYCHANGE SOME_FLAGS ,,
            MAYCHANGE [memory :> bytes(p3,128);
                       memory :> bytes(word_sub stackpointer (word 208),208)])`,
-  ARM_ADD_RETURN_STACK_TAC EDWARDS25519_PEPADD_EXEC
-    EDWARDS25519_PEPADD_CORRECT `[X19; X20]` 208);;
+  ARM_ADD_RETURN_STACK_TAC EDWARDS25519_EPADD_EXEC
+    EDWARDS25519_EPADD_CORRECT `[X19; X20]` 208);;
